@prefix : <http://www.semanticweb.org/CarterBenson/FutOn> .
@prefix dc: <http://purl.org/dc/elements/1.1/> .
@prefix obo: <http://purl.obolibrary.org/obo/> .
@prefix owl: <http://www.w3.org/2002/07/owl#> .
@prefix rdf: <http://www.w3.org/1999/02/22-rdf-syntax-ns#> .
@prefix xml: <http://www.w3.org/XML/1998/namespace> .
@prefix xsd: <http://www.w3.org/2001/XMLSchema#> .
@prefix rdfs: <http://www.w3.org/2000/01/rdf-schema#> .
@prefix skos: <http://www.w3.org/2004/02/skos/core#> .
@base <http://www.semanticweb.org/CarterBenson/FullFutOn> .

<http://www.semanticweb.org/CarterBenson/FullFutOn> rdf:type owl:Ontology ;
                                                     dc:contributor "Alec Sculley"@en ,
                                                                    "Austin Liebers"@en ,
                                                                    "Carter Benson"@en ,
                                                                    "John Beverley"@en ,
                                                                    "Katie Johnson"@en ;
                                                     rdfs:comment "This ontology is a provisional copy of FutOn, the Ontology of Football"@en ;
                                                     rdfs:label "FutOn"@en .

#################################################################
#    Annotation properties
#################################################################

###  http://purl.obolibrary.org/obo/IAO_0000115
obo:IAO_0000115 rdf:type owl:AnnotationProperty ;
                rdfs:label "defintion"@en .


###  http://purl.org/dc/elements/1.1/contributor
dc:contributor rdf:type owl:AnnotationProperty .


###  http://purl.org/dc/elements/1.1/identifier
dc:identifier rdf:type owl:AnnotationProperty .


###  http://purl.org/dc/elements/1.1/license
dc:license rdf:type owl:AnnotationProperty .


###  http://www.w3.org/2004/02/skos/core#altLabel
skos:altLabel rdf:type owl:AnnotationProperty .


###  http://www.w3.org/2004/02/skos/core#definition
skos:definition rdf:type owl:AnnotationProperty .


###  http://www.w3.org/2004/02/skos/core#example
skos:example rdf:type owl:AnnotationProperty .


###  http://www.w3.org/2004/02/skos/core#prefLabel
skos:prefLabel rdf:type owl:AnnotationProperty .


###  http://www.w3.org/2004/02/skos/core#scopeNote
skos:scopeNote rdf:type owl:AnnotationProperty .

#################################################################
#    Object Properties
#################################################################

###  http://purl.obolibrary.org/obo/BFO_0000054
obo:BFO_0000054 rdf:type owl:ObjectProperty ;
                owl:inverseOf obo:BFO_0000055 ;
                rdfs:domain obo:BFO_0000017 ;
                rdfs:range obo:BFO_0000015 ;
                dc:identifier "206-BFO" ;
                rdfs:label "has realization"@en ;
                skos:definition "b has realization c =Def c realizes b"@en ;
                skos:example "A disposition to go bald has realization a balding process, a role of student has realization a studying processes, the pumping function of a heart has realization a processes of pumping."@en ;
                skos:prefLabel "has realization"@en .


###  http://purl.obolibrary.org/obo/BFO_0000055
obo:BFO_0000055 rdf:type owl:ObjectProperty ;
                rdfs:domain obo:BFO_0000015 ;
                rdfs:range obo:BFO_0000017 ;
                dc:identifier "059-BFO" ;
                rdfs:label "realizes"@en ;
                skos:definition "(Elucidation) realizes is a relation between a process b and a realizable entity c such that inheres in some d and for all t, if b has participant d at t then c exists at t and the type instantiated by b is correlated with the type instantiated by c"@en ;
                skos:example "A balding process realizes a disposition to go bald, studying realizes a student role, a blood pumping process realizes the pumping function of a heart"@en ;
                skos:prefLabel "realizes"@en .


###  http://purl.obolibrary.org/obo/BFO_0000062
obo:BFO_0000062 rdf:type owl:ObjectProperty ;
                owl:inverseOf obo:BFO_0000063 ;
                rdf:type owl:TransitiveProperty ;
                rdfs:domain obo:BFO_0000003 ;
                rdfs:range obo:BFO_0000003 ;
                dc:identifier "213-BFO" ;
                rdfs:label "preceded by"@en ;
                skos:definition "b preceded by c =Def b precedes c"@en ;
                skos:example "The temporal region occupied by the second half of the match is preceded by the temporal region occupied by the first half of the match"@en ;
                skos:prefLabel "preceded by"@en .


###  http://purl.obolibrary.org/obo/BFO_0000063
obo:BFO_0000063 rdf:type owl:ObjectProperty ,
                         owl:TransitiveProperty ;
                rdfs:domain obo:BFO_0000003 ;
                rdfs:range obo:BFO_0000003 ;
                dc:identifier "270-BFO" ;
                rdfs:label "precedes"@en ;
                skos:definition "(Elucidation) precedes is a relation that holds between occurrents o, o' with respective temporal extents t, t', such that either the last instant of o is before the first instant of o' or the last instant of o is the first instant of o' and neither o nor o' are temporal instants"@en ;
                skos:example "The temporal region occupied by Mary's birth precedes the temporal region occupied by Mary's death"@en ;
                skos:prefLabel "precedes"@en ;
                skos:scopeNote "Each temporal region is its own temporal extent. The temporal extent of a spatiotemporal region is the temporal region it temporally projects onto. The temporal extent of a process or process boundary that occupies temporal region t is t."@en ,
                               "Precedes defines a strict partial order on occurrents."@en .


###  http://purl.obolibrary.org/obo/BFO_0000066
obo:BFO_0000066 rdf:type owl:ObjectProperty ;
                owl:inverseOf obo:BFO_0000183 ;
                rdfs:domain [ rdf:type owl:Class ;
                              owl:unionOf ( obo:BFO_0000015
                                            obo:BFO_0000035
                                          )
                            ] ;
                rdfs:range [ rdf:type owl:Class ;
                             owl:unionOf ( obo:BFO_0000029
                                           obo:BFO_0000040
                                         )
                           ] ;
                dc:identifier "143-BFO" ;
                rdfs:label "occurs in"@en ;
                skos:definition "b occurs in c =Def b is a process or a process boundary and c is a material entity or site, and for all t if b exists at t then c exists at t, b occupies a spatiotemporal region r that spatially projects onto spatial region s at t, c occupies spatial region s' at t, and s is continuant part of s' at t"@en ;
                skos:example "A process of digestion occurs in the interior of an organism, a process of loading artillery rounds into a tank cannon occurs in the interior of the tank"@en ;
                skos:prefLabel "occurs in"@en .


###  http://purl.obolibrary.org/obo/BFO_0000108
obo:BFO_0000108 rdf:type owl:ObjectProperty ;
                rdfs:domain [ rdf:type owl:Class ;
                              owl:unionOf ( obo:BFO_0000002
                                            obo:BFO_0000003
                                          )
                            ] ;
                rdfs:range obo:BFO_0000008 ;
                dc:identifier "118-BFO" ;
                rdfs:label "exists at"@en ;
                skos:definition "(Elucidation) exists at is a relation between a particular and some temporal region at which the particular exists"@en ;
                skos:example "First World War exists at 1914-1916, Mexico exists at January 1, 2000"@en ;
                skos:prefLabel "exists at"@en .


###  http://purl.obolibrary.org/obo/BFO_0000117
obo:BFO_0000117 rdf:type owl:ObjectProperty ;
                owl:inverseOf obo:BFO_0000132 ;
                rdf:type owl:TransitiveProperty ;
                rdfs:domain obo:BFO_0000003 ;
                rdfs:range obo:BFO_0000003 ;
                dc:identifier "202-BFO" ;
                rdfs:label "has occurrent part"@en ;
                skos:definition "(Elucidation) has occurrent part is a relation between an occurrent c and occurrent b when c is a part of b"@en ;
                skos:example "Mary's life has occurrent part Mary's 5th birthday"@en ;
                skos:prefLabel "has occurrent part"@en .


###  http://purl.obolibrary.org/obo/BFO_0000118
obo:BFO_0000118 rdf:type owl:ObjectProperty ;
                rdfs:subPropertyOf obo:BFO_0000117 ;
                owl:inverseOf obo:BFO_0000138 ;
                rdf:type owl:TransitiveProperty ;
                rdfs:domain obo:BFO_0000003 ;
                rdfs:range obo:BFO_0000003 ;
                dc:identifier "154-BFO" ;
                rdfs:label "has proper occurrent part"@en ;
                skos:definition "b has proper occurrent part c =Def b has occurrent part c and b and c are not identical"@en ;
                skos:example "As for has occurrent part"@en ;
                skos:prefLabel "has proper occurrent part"@en .


###  http://purl.obolibrary.org/obo/BFO_0000121
obo:BFO_0000121 rdf:type owl:ObjectProperty ;
                rdfs:subPropertyOf obo:BFO_0000117 ;
                owl:inverseOf obo:BFO_0000139 ;
                rdf:type owl:TransitiveProperty ;
                rdfs:domain obo:BFO_0000003 ;
                rdfs:range obo:BFO_0000003 ;
                dc:identifier "211-BFO" ;
                rdfs:label "has temporal part"@en ;
                skos:definition "b has temporal part c =Def c temporal part of b"@en ;
                skos:example "Your life has temporal part the first year of your life"@en ;
                skos:prefLabel "has temporal part"@en .


###  http://purl.obolibrary.org/obo/BFO_0000132
obo:BFO_0000132 rdf:type owl:ObjectProperty ,
                         owl:TransitiveProperty ;
                rdfs:domain obo:BFO_0000003 ;
                rdfs:range obo:BFO_0000003 ;
                dc:identifier "003-BFO" ;
                rdfs:label "occurrent part of"@en ;
                skos:definition "(Elucidation) b occurrent part of c =Def c has occurrent part b"@en ;
                skos:example "Mary's 5th birthday is an occurrent part of Mary's life, the first set of the tennis match is an occurrent part of the tennis match"@en ;
                skos:prefLabel "occurrent part of"@en .


###  http://purl.obolibrary.org/obo/BFO_0000136
obo:BFO_0000136 rdf:type owl:ObjectProperty ;
                rdfs:subPropertyOf obo:BFO_0000139 ;
                owl:inverseOf obo:BFO_0000181 ;
                rdfs:domain obo:BFO_0000003 ;
                rdfs:range obo:BFO_0000003 ;
                dc:identifier "116-BFO" ;
                rdfs:label "proper temporal part of"@en ;
                skos:definition "b proper temporal part of c =Def b temporal part of c and b and c are not identical"@en ;
                skos:example "As for temporal part of"@en ;
                skos:prefLabel "proper temporal part of"@en .


###  http://purl.obolibrary.org/obo/BFO_0000138
obo:BFO_0000138 rdf:type owl:ObjectProperty ;
                rdfs:subPropertyOf obo:BFO_0000132 ;
                rdf:type owl:TransitiveProperty ;
                rdfs:domain obo:BFO_0000003 ;
                rdfs:range obo:BFO_0000003 ;
                dc:identifier "005-BFO" ;
                rdfs:label "proper occurrent part of"@en ;
                skos:definition "b proper occurrent part of c =Def b occurrent part of c & b and c are not identical"@en ;
                skos:example "As for occurrent part of"@en ;
                skos:prefLabel "proper occurrent part of"@en .


###  http://purl.obolibrary.org/obo/BFO_0000139
obo:BFO_0000139 rdf:type owl:ObjectProperty ;
                rdfs:subPropertyOf obo:BFO_0000132 ;
                rdf:type owl:TransitiveProperty ;
                rdfs:domain obo:BFO_0000003 ;
                rdfs:range obo:BFO_0000003 ;
                dc:identifier "078-BFO" ;
                rdfs:label "temporal part of"@en ;
                skos:definition "b temporal part of c =Def b occurrent part of c and either b and c are temporal regions or b and c are spatiotemporal regions, b temporally projects onto an occurrent part of the temporal region that c temporally projects onto or b and c are processes or process boundaries and b occupies a temporal region that is an occurrent part of the temporal region that c occupies"@en ;
                skos:example "Your heart beating from 4pm to 5pm today is a temporal part of the process of your heart beating, the 4th year of your life is a temporal part of your life, as is the process boundary which separates the 3rd and 4th years of your life, the first quarter of a game of football is a temporal part of the whole game"@en ;
                skos:prefLabel "temporal part of"@en .


###  http://purl.obolibrary.org/obo/BFO_0000153
obo:BFO_0000153 rdf:type owl:ObjectProperty ,
                         owl:FunctionalProperty ;
                rdfs:domain obo:BFO_0000011 ;
                rdfs:range obo:BFO_0000008 ;
                dc:identifier "080-BFO" ;
                rdfs:label "temporally projects onto"@en ;
                skos:definition "(Elucidation) temporally projects onto is a relation between a spatiotemporal region and some temporal region which is its temporal extent"@en ;
                skos:example "The world line of a particle temporally projects onto the temporal region extending from the beginning to the end of the existence of the particle"@en ;
                skos:prefLabel "temporally projects onto"@en .


###  http://purl.obolibrary.org/obo/BFO_0000181
obo:BFO_0000181 rdf:type owl:ObjectProperty ;
                rdfs:subPropertyOf obo:BFO_0000121 ;
                rdfs:domain obo:BFO_0000003 ;
                rdfs:range obo:BFO_0000003 ;
                dc:identifier "212-BFO" ;
                rdfs:label "has proper temporal part"@en ;
                skos:definition "b has proper temporal part c =Def c proper temporal part of b"@en ;
                skos:example "As for has temporal part"@en ;
                skos:prefLabel "has proper temporal part"@en .


###  http://purl.obolibrary.org/obo/BFO_0000183
obo:BFO_0000183 rdf:type owl:ObjectProperty ;
                rdfs:domain [ rdf:type owl:Class ;
                              owl:unionOf ( obo:BFO_0000029
                                            obo:BFO_0000040
                                          )
                            ] ;
                rdfs:range [ rdf:type owl:Class ;
                             owl:unionOf ( obo:BFO_0000015
                                           obo:BFO_0000035
                                         )
                           ] ;
                dc:identifier "267-BFO" ;
                rdfs:label "environs"@en ;
                skos:definition "b environs c =Def c occurs in b"@en ;
                skos:example "A mouth environs a process of mastication, a city environs traffic"@en ;
                skos:prefLabel "environs"@en .


###  http://purl.obolibrary.org/obo/BFO_0000184
obo:BFO_0000184 rdf:type owl:ObjectProperty ;
                owl:inverseOf obo:BFO_0000185 ;
                rdf:type owl:FunctionalProperty ,
                         owl:InverseFunctionalProperty ;
                rdfs:domain obo:BFO_0000182 ;
                rdfs:range obo:BFO_0000040 ;
                dc:identifier "144-BFO" ;
                rdfs:label "history of"@en ;
                skos:definition "(Elucidation) history of is a relation between a history b and a material entity c when b is the unique history of c"@en ;
                skos:example "This life is the history of this organism"@en ;
                skos:prefLabel "history of"@en .


###  http://purl.obolibrary.org/obo/BFO_0000185
obo:BFO_0000185 rdf:type owl:ObjectProperty ;
                rdfs:domain obo:BFO_0000040 ;
                rdfs:range obo:BFO_0000182 ;
                dc:identifier "145-BFO" ;
                rdfs:label "has history"@en ;
                skos:definition "b has history c =Def c history of b"@en ;
                skos:example "This organism has history this life"@en ;
                skos:prefLabel "has history"@en .


###  http://purl.obolibrary.org/obo/BFO_0000194
obo:BFO_0000194 rdf:type owl:ObjectProperty ;
                owl:inverseOf obo:BFO_0000195 ;
                rdfs:domain [ rdf:type owl:Class ;
                              owl:unionOf ( obo:BFO_0000020
                                            [ owl:intersectionOf ( obo:BFO_0000004
                                                                   [ rdf:type owl:Class ;
                                                                     owl:complementOf obo:BFO_0000006
                                                                   ]
                                                                 ) ;
                                              rdf:type owl:Class
                                            ]
                                          )
                            ] ;
                rdfs:range obo:BFO_0000020 ;
                dc:identifier "260-BFO" ;
                rdfs:label "specifically depended on by"@en ;
                skos:altLabel "s-depended on by"@en ;
                skos:definition "b s-depended on by c =Def c specifically depends on b"@en ;
                skos:example "A tomato is s-depended on a redness quality"@en ;
                skos:prefLabel "specifically depended on by"@en .


###  http://purl.obolibrary.org/obo/BFO_0000195
obo:BFO_0000195 rdf:type owl:ObjectProperty ;
                rdfs:domain obo:BFO_0000020 ;
                rdfs:range [ rdf:type owl:Class ;
                             owl:unionOf ( obo:BFO_0000020
                                           [ owl:intersectionOf ( obo:BFO_0000004
                                                                  [ rdf:type owl:Class ;
                                                                    owl:complementOf obo:BFO_0000006
                                                                  ]
                                                                ) ;
                                             rdf:type owl:Class
                                           ]
                                         )
                           ] ;
                dc:identifier "012-BFO" ;
                rdfs:label "specifically depends on"@en ;
                skos:altLabel "s-depends on"@en ;
                skos:definition "(Elucidation) specifically depends is a relation between a specifically dependent continuant b and and a specifically dependent continuant or independent continuant that is not a spatial region c, such that b and c do not share common parts, b is of a nature such that at all times t it cannot exist at t unless c exists at t, and b is not a boundary of c"@en ;
                skos:example "A shape s-depends on the shaped object, hue, saturation and brightness of a colour sample s-depend on each other"@en ;
                skos:prefLabel "specifically depends on"@en ;
                skos:scopeNote "The analogue of s-dependence for occurrents is has participant."@en .


###  http://purl.obolibrary.org/obo/BFO_0000196
obo:BFO_0000196 rdf:type owl:ObjectProperty ;
                rdfs:subPropertyOf obo:BFO_0000194 ;
                owl:inverseOf obo:BFO_0000197 ;
                rdfs:domain [ owl:intersectionOf ( obo:BFO_0000004
                                                   [ rdf:type owl:Class ;
                                                     owl:complementOf obo:BFO_0000006
                                                   ]
                                                 ) ;
                              rdf:type owl:Class
                            ] ;
                rdfs:range obo:BFO_0000020 ;
                dc:identifier "053-BFO" ;
                rdfs:label "bearer of"@en ;
                skos:definition "b bearer of c =Def c inheres in b"@en ;
                skos:example "A patch of ink is the bearer of a colour quality, an organism is the bearer of a temperature quality"@en ;
                skos:prefLabel "bearer of"@en .


###  http://purl.obolibrary.org/obo/BFO_0000197
obo:BFO_0000197 rdf:type owl:ObjectProperty ;
                rdfs:subPropertyOf obo:BFO_0000195 ;
                rdfs:domain obo:BFO_0000020 ;
                rdfs:range [ owl:intersectionOf ( obo:BFO_0000004
                                                  [ rdf:type owl:Class ;
                                                    owl:complementOf obo:BFO_0000006
                                                  ]
                                                ) ;
                             rdf:type owl:Class
                           ] ;
                dc:identifier "051-BFO" ;
                rdfs:label "inheres in"@en ;
                skos:definition "b inheres in c =Def b is a specifically dependent continuant and c is an independent continuant that is not a spatial region and b s-depends on c"@en ;
                skos:example "A shape inheres in a shaped object, a mass inheres in a material entity"@en ;
                skos:prefLabel "inheres in"@en .


###  http://purl.obolibrary.org/obo/BFO_0000199
obo:BFO_0000199 rdf:type owl:ObjectProperty ,
                         owl:FunctionalProperty ;
                rdfs:domain [ rdf:type owl:Class ;
                              owl:unionOf ( obo:BFO_0000015
                                            obo:BFO_0000035
                                          )
                            ] ;
                rdfs:range obo:BFO_0000008 ;
                dc:identifier "132-BFO" ;
                rdfs:label "occupies temporal region"@en ;
                skos:definition "process or process boundary p occupies temporal region t =Def the spatiotemporal region occupied by p temporally projects onto t"@en ;
                skos:example "The Second World War occupies the temporal region September 1, 1939 - September 2, 1945"@en ;
                skos:prefLabel "occupies temporal region"@en .


###  http://purl.obolibrary.org/obo/BFO_0000200
obo:BFO_0000200 rdf:type owl:ObjectProperty ,
                         owl:FunctionalProperty ;
                rdfs:domain [ rdf:type owl:Class ;
                              owl:unionOf ( obo:BFO_0000015
                                            obo:BFO_0000035
                                          )
                            ] ;
                rdfs:range obo:BFO_0000011 ;
                dc:identifier "082-BFO" ;
                rdfs:label "occupies spatiotemporal region"@en ;
                skos:definition "(Elucidation) occupies spatiotemporal region is a relation between a process or process boundary and the spatiotemporal region which is its spatiotemporal extent"@en ;
                skos:example "A particle emitted by a nuclear reactor occupies the spatiotemporal region which is its trajectory"@en ;
                skos:prefLabel "occupies spatiotemporal region"@en .


###  http://purl.obolibrary.org/obo/BFO_0000221
obo:BFO_0000221 rdf:type owl:ObjectProperty ;
                owl:inverseOf obo:BFO_0000222 ;
                rdfs:domain obo:BFO_0000203 ;
                rdfs:range obo:BFO_0000008 ;
                dc:identifier "268-BFO" ;
                rdfs:label "first instant of"@en ;
                skos:definition "temporal instant t first instant of temporal region t' =Def t precedes all temporal parts of t' other than t"@en ;
                skos:example "An hour starting at midnight yesterday has first instant midnight yesterday"@en ;
                skos:prefLabel "first instant of"@en .


###  http://purl.obolibrary.org/obo/BFO_0000222
obo:BFO_0000222 rdf:type owl:ObjectProperty ,
                         owl:FunctionalProperty ;
                rdfs:domain obo:BFO_0000008 ;
                rdfs:range obo:BFO_0000203 ;
                dc:identifier "261-BFO" ;
                rdfs:label "has first instant"@en ;
                skos:definition "t has first instant t' =Def t' first instant of t"@en ;
                skos:example "The first hour of a year has first instant midnight on December 31"@en ;
                skos:prefLabel "has first instant"@en .


###  http://purl.obolibrary.org/obo/BFO_0000223
obo:BFO_0000223 rdf:type owl:ObjectProperty ;
                owl:inverseOf obo:BFO_0000224 ;
                rdfs:domain obo:BFO_0000203 ;
                rdfs:range obo:BFO_0000008 ;
                dc:identifier "269-BFO" ;
                rdfs:label "last instant of"@en ;
                skos:definition "temporal instant t last instant of temporal region t' =Def all temporal parts of t' other than t precede t"@en ;
                skos:example "Last midnight is the last instant of yesterday"@en ;
                skos:prefLabel "last instant of"@en .


###  http://purl.obolibrary.org/obo/BFO_0000224
obo:BFO_0000224 rdf:type owl:ObjectProperty ,
                         owl:FunctionalProperty ;
                rdfs:domain obo:BFO_0000008 ;
                rdfs:range obo:BFO_0000203 ;
                dc:identifier "215-BFO" ;
                rdfs:label "has last instant"@en ;
                skos:definition "t has last instant t' =Def t' last instant of t"@en ;
                skos:example "The last hour of a year has last instant midnight December 31"@en ;
                skos:prefLabel "has last instant"@en .


#################################################################
#    Classes
#################################################################

###  http://www.ontologyrepository.com/CommonCoreOntologies/ActionPermission
<http://www.ontologyrepository.com/CommonCoreOntologies/ActionPermission> rdf:type owl:Class ;
                                                                          rdfs:subClassOf <http://www.ontologyrepository.com/CommonCoreOntologies/ActionRegulation> ;
                                                                          obo:IAO_0000115 "An Action Regulation that permits some Act."@en ;
                                                                          rdfs:label "Action Permission"@en .


###  http://www.ontologyrepository.com/CommonCoreOntologies/ActionProhibition
<http://www.ontologyrepository.com/CommonCoreOntologies/ActionProhibition> rdf:type owl:Class ;
                                                                           rdfs:subClassOf <http://www.ontologyrepository.com/CommonCoreOntologies/ActionRegulation> ;
                                                                           obo:IAO_0000115 "An Action Regulation that prohibits some Act."@en ;
                                                                           rdfs:label "Action Prohibition"@en .


###  http://www.ontologyrepository.com/CommonCoreOntologies/ActionRegulation
<http://www.ontologyrepository.com/CommonCoreOntologies/ActionRegulation> rdf:type owl:Class ;
                                                                          rdfs:subClassOf <http://www.ontologyrepository.com/CommonCoreOntologies/DirectiveInformationContentEntity> ;
                                                                          obo:IAO_0000115 "A Directive Information Content Entity that prescribes an Act as required, prohibited, or permitted, and is the output of an Act which realizes some Authority Role."@en ,
                                                                                          "Action Regulation"@en .


###  http://www.ontologyrepository.com/CommonCoreOntologies/ActionRequirement
<http://www.ontologyrepository.com/CommonCoreOntologies/ActionRequirement> rdf:type owl:Class ;
                                                                           rdfs:subClassOf <http://www.ontologyrepository.com/CommonCoreOntologies/ActionRegulation> ;
                                                                           obo:IAO_0000115 "An Action Regulation that requires some Act."@en ;
                                                                           rdfs:label "Action Requirement"@en .


###  http://www.ontologyrepository.com/CommonCoreOntologies/Algorithm
<http://www.ontologyrepository.com/CommonCoreOntologies/Algorithm> rdf:type owl:Class ;
                                                                   rdfs:subClassOf <http://www.ontologyrepository.com/CommonCoreOntologies/DirectiveInformationContentEntity> ;
                                                                   obo:IAO_0000115 "A Directive Information Content Entity that prescribes the inputs and output of mathematical functions as well as workflow of execution for achieving a predefined objective"@en ;
                                                                   rdfs:label "Algorithm" .


###  http://www.ontologyrepository.com/CommonCoreOntologies/DescriptiveInformationContentEntity
<http://www.ontologyrepository.com/CommonCoreOntologies/DescriptiveInformationContentEntity> rdf:type owl:Class ;
                                                                                             obo:IAO_0000115 "An Information Content Entity that consists of a set of propositions that describe some Entity."@en ;
                                                                                             rdfs:label "Descriptive Information Content Entity"@en .


###  http://www.ontologyrepository.com/CommonCoreOntologies/DirectiveInformationContentEntity
<http://www.ontologyrepository.com/CommonCoreOntologies/DirectiveInformationContentEntity> rdf:type owl:Class ;
                                                                                           obo:IAO_0000115 "An Information Content Entity that consists of a set of propositions or images (as in the case of a blueprint) that prescribe some Entity."@en ;
                                                                                           rdfs:label "Directive Information Content Entity"@en .


###  http://www.ontologyrepository.com/CommonCoreOntologies/Ideology
<http://www.ontologyrepository.com/CommonCoreOntologies/Ideology> rdf:type owl:Class ;
                                                                  obo:IAO_0000115 "An Information Content Entity that consists of a collection of claims about how some part of the world is or should be and which is accepted as true by an Agent or Group of Agents such that it forms the basis of their beliefs, goals, expectations, and motivations."@en ;
                                                                  rdfs:label "Ideology" .


###  http://www.ontologyrepository.com/CommonCoreOntologies/IntentionalAct
<http://www.ontologyrepository.com/CommonCoreOntologies/IntentionalAct> rdf:type owl:Class ;
                                                                        obo:IAO_0000115 "An Act in which at least one Agent plays a causative role and which is prescribed by some Directive Information Content Entity held by at least one of the Agents."@en ;
                                                                        rdfs:label "Planned Act" .


###  http://www.ontologyrepository.com/CommonCoreOntologies/MeasurementInformationContentEntity
<http://www.ontologyrepository.com/CommonCoreOntologies/MeasurementInformationContentEntity> rdf:type owl:Class ;
                                                                                             rdfs:subClassOf <http://www.ontologyrepository.com/CommonCoreOntologies/DescriptiveInformationContentEntity> ;
                                                                                             obo:IAO_0000115 "A Descriptive Information Content Entity that describes the extent, dimensions, quantity, or quality of an Entity relative to some standard."@en ;
                                                                                             rdfs:label "Measurement Information Content Entity" .


###  http://www.ontologyrepository.com/CommonCoreOntologies/OccupationRole
<http://www.ontologyrepository.com/CommonCoreOntologies/OccupationRole> rdf:type owl:Class ;
                                                                        obo:IAO_0000115 "A Role that inheres in an Agent in virtue of the responsibilities that Agent is expected to fulfill within the context of some Act of Employment."@en ;
                                                                        rdfs:label "Occupation Role"@en .


###  http://www.ontologyrepository.com/CommonCoreOntologies/PredictiveInformationContentEntity
<http://www.ontologyrepository.com/CommonCoreOntologies/PredictiveInformationContentEntity> rdf:type owl:Class ;
                                                                                            rdfs:subClassOf <http://www.ontologyrepository.com/CommonCoreOntologies/DescriptiveInformationContentEntity> ;
                                                                                            obo:IAO_0000115 "A Descriptive Information Content Entity that describes an uncertain future event."@en ;
                                                                                            rdfs:label "PredictiveInformationContentEntity" .


###  http://www.semanticweb.org/CarterBenson/FutOn00113
<http://www.semanticweb.org/CarterBenson/FutOn00113> rdf:type owl:Class ;
                                                     rdfs:subClassOf :FutOn_00004 ;
                                                     obo:IAO_0000115 "A playerAct that represents any action intentionally performed by a substitute player or non-playing athlete from the bench during a match."@en ;
                                                     rdfs:label "benchPlayerAct"@en .


###  http://www.semanticweb.org/CarterBenson/FutOn00114
<http://www.semanticweb.org/CarterBenson/FutOn00114> rdf:type owl:Class ;
                                                     rdfs:subClassOf <http://www.semanticweb.org/CarterBenson/FutOn00113> ;
                                                     obo:IAO_0000115 "A BenchPlayerAct that involves a substitute player or non-playing athlete vocally encouraging their team from the sidelines. This can include cheering, chanting, or offering positive affirmations."@en ;
                                                     rdfs:label "benchPlayerCheeringAct"@en .


###  http://www.semanticweb.org/CarterBenson/FutOn00115
<http://www.semanticweb.org/CarterBenson/FutOn00115> rdf:type owl:Class ;
                                                     rdfs:subClassOf <http://www.semanticweb.org/CarterBenson/FutOn00113> ;
                                                     obo:IAO_0000115 "A BenchPlayerAct that involves a substitute player or non-playing athlete engaging in conversations about game tactics and strategies with other bench members or coaches."@en ;
                                                     rdfs:label "benchPlayerStrategicDiscussionAct"@en .


###  http://www.semanticweb.org/CarterBenson/FutOn00116
<http://www.semanticweb.org/CarterBenson/FutOn00116> rdf:type owl:Class ;
                                                     rdfs:subClassOf <http://www.semanticweb.org/CarterBenson/FutOn00113> ;
                                                     obo:IAO_0000115 "A BenchPlayerAct that involves a substitute player or non-playing athlete performing physical activity to prepare for potential entry into the match. This can include activities like stretching, jogging, and sport-specific drills."@en ;
                                                     rdfs:label "benchPlayerWarmUpAct"@en .


###  http://www.semanticweb.org/CarterBenson/FutOn00117
<http://www.semanticweb.org/CarterBenson/FutOn00117> rdf:type owl:Class ;
                                                     rdfs:subClassOf <http://www.semanticweb.org/CarterBenson/FutOn00113> ;
                                                     obo:IAO_0000115 "A BenchPlayerAct that involves a substitute player or non-playing athlete assisting the coaching staff in various ways, such as relaying messages to on-field players or contributing to tactical decisions."@en ;
                                                     rdfs:label "benchPlayerCoachingAssistanceAct"@en .


###  http://www.semanticweb.org/CarterBenson/FutOn00118
<http://www.semanticweb.org/CarterBenson/FutOn00118> rdf:type owl:Class ;
                                                     rdfs:subClassOf <http://www.semanticweb.org/CarterBenson/FutOn00113> ;
                                                     obo:IAO_0000115 "A BenchPlayerAct that involves a substitute player or non-playing athlete preparing to enter the match as a substitute, often in response to a coach's decision or a teammate's injury."@en ;
                                                     rdfs:label "benchPlayerSubstitutionReadinessAct"@en .


###  http://www.semanticweb.org/CarterBenson/FutOn00119
<http://www.semanticweb.org/CarterBenson/FutOn00119> rdf:type owl:Class ;
                                                     rdfs:subClassOf <http://www.semanticweb.org/CarterBenson/FutOn00113> ;
                                                     obo:IAO_0000115 "A BenchPlayerAct that involves a substitute player or non-playing athlete consuming fluids to maintain hydration levels during the match."@en ;
                                                     rdfs:label "benchPlayerRehydrationAct"@en .


###  http://www.semanticweb.org/CarterBenson/FutOn00120
<http://www.semanticweb.org/CarterBenson/FutOn00120> rdf:type owl:Class ;
                                                     rdfs:subClassOf <http://www.semanticweb.org/CarterBenson/FutOn00113> ;
                                                     obo:IAO_0000115 "A BenchPlayerAct that involves a substitute player or non-playing athlete consuming energy-dense foods or supplements to maintain energy levels and readiness for potential match entry."@en ;
                                                     rdfs:label "benchPlayerNutritionAct"@en .


###  http://www.semanticweb.org/CarterBenson/FutOn00121
<http://www.semanticweb.org/CarterBenson/FutOn00121> rdf:type owl:Class ;
                                                     rdfs:subClassOf <http://www.semanticweb.org/CarterBenson/FutOnFutOn:00001> ;
                                                     obo:IAO_0000115 "An intentionalMatchAct that represents any action deliberately performed by an individual spectator during a match."@en ;
                                                     rdfs:label "fanAct"@en .


###  http://www.semanticweb.org/CarterBenson/FutOn00122
<http://www.semanticweb.org/CarterBenson/FutOn00122> rdf:type owl:Class ;
                                                     rdfs:subClassOf <http://www.semanticweb.org/CarterBenson/FutOn00121> ;
                                                     obo:IAO_0000115 "A fanAct that involves vocal support, often in the form of shouting, chanting, or singing, aimed at encouraging a team or player."@en ;
                                                     rdfs:label "cheeringAct"@en .


###  http://www.semanticweb.org/CarterBenson/FutOn00123
<http://www.semanticweb.org/CarterBenson/FutOn00123> rdf:type owl:Class ;
                                                     rdfs:subClassOf <http://www.semanticweb.org/CarterBenson/FutOn00121> ;
                                                     obo:IAO_0000115 "A fanAct that involves clapping hands to express approval, praise, or enthusiasm for a specific play or player."@en ;
                                                     rdfs:label "applaudingAct"@en .


###  http://www.semanticweb.org/CarterBenson/FutOn00124
<http://www.semanticweb.org/CarterBenson/FutOn00124> rdf:type owl:Class ;
                                                     rdfs:subClassOf <http://www.semanticweb.org/CarterBenson/FutOn00121> ;
                                                     obo:IAO_0000115 "A fanAct that involves creating and showing banners or signs, usually to express support for a team or player, or to communicate a particular sentiment or message."@en ;
                                                     rdfs:label "bannerDisplayingAct"@en .


###  http://www.semanticweb.org/CarterBenson/FutOn00125
<http://www.semanticweb.org/CarterBenson/FutOn00125> rdf:type owl:Class ;
                                                     rdfs:subClassOf <http://www.semanticweb.org/CarterBenson/FutOn00121> ;
                                                     obo:IAO_0000115 "A fanAct that involves posting on social media platforms about the match, typically to share views, express support, or engage with other fans."@en ;
                                                     rdfs:label "socialMediaPostingAct"@en .


###  http://www.semanticweb.org/CarterBenson/FutOn00126
<http://www.semanticweb.org/CarterBenson/FutOn00126> rdf:type owl:Class ;
                                                     rdfs:subClassOf <http://www.semanticweb.org/CarterBenson/FutOn00121> ;
                                                     obo:IAO_0000115 "A fanAct that involves expressing disapproval or discontent, typically towards a particular player, team, or referee decision, by booing or jeering."@en ;
                                                     rdfs:label "booingAct"@en .


###  http://www.semanticweb.org/CarterBenson/FutOn00127
<http://www.semanticweb.org/CarterBenson/FutOn00127> rdf:type owl:Class ;
                                                     rdfs:subClassOf <http://www.semanticweb.org/CarterBenson/FutOn00121> ;
                                                     obo:IAO_0000115 "A fanAct that involves intentional silence or non-participation in certain activities (like chants or applause) to express dissatisfaction or protest against an issue related to the match or the teams."@en ;
                                                     rdfs:label "silentProtestAct"@en .


###  http://www.semanticweb.org/CarterBenson/FutOn00128
<http://www.semanticweb.org/CarterBenson/FutOn00128> rdf:type owl:Class ;
                                                     rdfs:subClassOf <http://www.semanticweb.org/CarterBenson/FutOn00121> ;
                                                     obo:IAO_0000115 "A fanAct that involves a spectator unlawfully entering the playing area during a match. This is generally considered dangerous and disrespectful, and it's usually strictly prohibited."@en ;
                                                     rdfs:label "pitchInvasionAct"@en .


###  http://www.semanticweb.org/CarterBenson/FutOn00129
<http://www.semanticweb.org/CarterBenson/FutOn00129> rdf:type owl:Class ;
                                                     rdfs:subClassOf <http://www.semanticweb.org/CarterBenson/FutOn00121> ;
                                                     obo:IAO_0000115 "A fanAct that involves violent, disorderly, or destructive behavior, often resulting in harm to others or damage to property."@en ;
                                                     rdfs:label "hooliganismAct"@en .


###  http://www.semanticweb.org/CarterBenson/FutOn00130
<http://www.semanticweb.org/CarterBenson/FutOn00130> rdf:type owl:Class ;
                                                     rdfs:subClassOf <http://www.semanticweb.org/CarterBenson/FutOn00121> ;
                                                     obo:IAO_0000115 "A fanAct that involves offensive, discriminatory, or hate-fueled chants or shouts. This can include racism, sexism, homophobia, and other forms of abuse."@en ;
                                                     rdfs:label "abusiveChantingAct"@en .


###  http://www.semanticweb.org/CarterBenson/FutOn00131
<http://www.semanticweb.org/CarterBenson/FutOn00131> rdf:type owl:Class ;
                                                     rdfs:subClassOf <http://www.semanticweb.org/CarterBenson/FutOn00121> ;
                                                     obo:IAO_0000115 "A fanAct that involves throwing objects onto the pitch or at other spectators. This can be very dangerous and is usually strictly prohibited."@en ;
                                                     rdfs:label "projectileThrowingAct"@en .


###  http://www.semanticweb.org/CarterBenson/FutOn00132
<http://www.semanticweb.org/CarterBenson/FutOn00132> rdf:type owl:Class ;
                                                     rdfs:subClassOf <http://www.semanticweb.org/CarterBenson/FutOn00121> ;
                                                     obo:IAO_0000115 "A fanAct that involves the intentional discomfort or harm of others through unwanted actions or behaviors, such as stalking or physical and verbal abuse."@en ;
                                                     rdfs:label "harassmentAct"@en .


###  http://www.semanticweb.org/CarterBenson/FutOn00133
<http://www.semanticweb.org/CarterBenson/FutOn00133> rdf:type owl:Class ;
                                                     rdfs:subClassOf <http://www.semanticweb.org/CarterBenson/FutOn00121> ;
                                                     obo:IAO_0000115 "A fanAct that involves the deliberate damage or defacement of property, whether the venue's facilities, vehicles in the vicinity, or other fans' belongings."@en ;
                                                     rdfs:label "vandalismAct"@en .


###  http://www.semanticweb.org/CarterBenson/FutOnFutOn_00002
:FutOn_00002 rdf:type owl:Class ;
             rdfs:subClassOf <http://www.semanticweb.org/CarterBenson/FutOnFutOn:00001> ;
             obo:IAO_0000115 "an intentionalMatchAct that represents any action deliberately performed by a referee during amatch."@en ;
             rdfs:comment "These actions can include making decisions on rule infractions, starting and stopping play, time-keeping, and any other actions aimed at enforcing the rules of thematch and ensuring fair play."@en ;
             rdfs:label "refereeAct"@en .


###  http://www.semanticweb.org/CarterBenson/FutOnFutOn_00003
:FutOn_00003 rdf:type owl:Class ;
             rdfs:subClassOf <http://www.semanticweb.org/CarterBenson/FutOnFutOn:00001> ;
             obo:IAO_0000115 "an intentionalMatchAct that represents any action deliberately performed by a team's manager or coach during amatch."@en ;
             rdfs:comment "These actions can include strategic decisions, substitutions, tactical instructions, and any other actions aimed at guiding the team's play and strategy."@en ;
             rdfs:label "managerAct"@en .


###  http://www.semanticweb.org/CarterBenson/FutOnFutOn_00004
:FutOn_00004 rdf:type owl:Class ;
             rdfs:subClassOf <http://www.semanticweb.org/CarterBenson/FutOnFutOn:00001> ;
             obo:IAO_0000115 "an intentionalMatchAct that represents any action performed intentionally by a player during amatch."@en ;
             rdfs:label "playerAct"@en .


###  http://www.semanticweb.org/CarterBenson/FutOnFutOn_00005
:FutOn_00005 rdf:type owl:Class ;
             rdfs:subClassOf :FutOn_00151 ;
             obo:IAO_0000115 "is a playerAct that involves actions taken by a player when their team does not have control of the ball."@en ;
             rdfs:label "outOfPossessionAct"@en .


###  http://www.semanticweb.org/CarterBenson/FutOnFutOn_00006
:FutOn_00006 rdf:type owl:Class ;
             rdfs:subClassOf :FutOn_00005 ;
             obo:IAO_0000115 "an outOfPossessionAct, that involves a player positioning themselves close to a specific opposing player with the intent of limiting their influence on thematch by preventing them from receiving the ball or obstructing their plays when they do have the ball,"@en ;
             rdfs:label "markingAct"@en .


###  http://www.semanticweb.org/CarterBenson/FutOnFutOn_00007
:FutOn_00007 rdf:type owl:Class ;
             rdfs:subClassOf :FutOn_00006 ;
             obo:IAO_0000115 "is a markingAct where a defender is responsible for guarding a specific area of the pitch, rather than a specific player. The defender attempts to intercept any opponent or ball that enters their zone."@en ;
             rdfs:label "manMarkingAct"@en .


###  http://www.semanticweb.org/CarterBenson/FutOnFutOn_00008
:FutOn_00008 rdf:type owl:Class ;
             rdfs:subClassOf :FutOn_00006 ;
             obo:IAO_0000115 "a markingAct where a defender is assigned a specific player from the opposing team to guard, with the intent to limit their influence on thematch. The defender typically shadows their assigned player, staying close and attempting to disrupt their play."@en ;
             rdfs:label "zonalMarkingAct"@en .


###  http://www.semanticweb.org/CarterBenson/FutOnFutOn_00009
:FutOn_00009 rdf:type owl:Class ;
             rdfs:subClassOf :FutOn_00005 ;
             obo:IAO_0000115 "an outOfPossessionAct that is performed by a player when they attempt to dispossess an opponent by physically challenging them for the ball."@en ;
             rdfs:label "tackleAct"@en .


###  http://www.semanticweb.org/CarterBenson/FutOnFutOn_00010
:FutOn_00010 rdf:type owl:Class ;
             rdfs:subClassOf :FutOn_00009 ;
             obo:IAO_0000115 "a tackleAct that is performed by a player when they position themselves in the path of the ball, typically while it is being shot or passed by an opponent, in an attempt to stop its progress or change its direction."@en ;
             rdfs:label "blockTackleAct"@en .


###  http://www.semanticweb.org/CarterBenson/FutOnFutOn_00011
:FutOn_00011 rdf:type owl:Class ;
             rdfs:subClassOf :FutOn_00009 ;
             obo:IAO_0000115 "a tackleAct that is performed by a player when they slide on the ground to challenge an opponent for the ball, typically with one leg extended."@en ;
             rdfs:label "slideTackleAct"@en .


###  http://www.semanticweb.org/CarterBenson/FutOnFutOn_00012
:FutOn_00012 rdf:type owl:Class ;
             rdfs:subClassOf :FutOn_00005 ;
             obo:IAO_0000115 "an outOfPossessionAct that is performed by a player when they disrupt an opponent's pass by moving into the ball's path, thereby gaining possession for their own team."@en ;
             rdfs:label "interceptionAct"@en .


###  http://www.semanticweb.org/CarterBenson/FutOnFutOn_00013
:FutOn_00013 rdf:type owl:Class ;
             rdfs:subClassOf :FutOn_00151 ;
             obo:IAO_0000115 "inPossessionAct is a playerAct that involves actions executed by players of the team that currently has control of the ball."@en ;
             rdfs:label "inPossessionAct"@en .


###  http://www.semanticweb.org/CarterBenson/FutOnFutOn_00014
:FutOn_00014 rdf:type owl:Class ;
             rdfs:subClassOf :FutOn_00112 ;
             obo:IAO_0000115 "rotationAct is an offBallAct that involves the strategic movement of a player who does not directly control the ball."@en ;
             rdfs:label "rotationAct"@en .


###  http://www.semanticweb.org/CarterBenson/FutOnFutOn_00015
:FutOn_00015 rdf:type owl:Class ;
             rdfs:subClassOf :FutOn_00014 ;
             obo:IAO_0000115 "symmetricalRotationAct in football is a rotationAct that describes a strategic movement or action in which players rotate and change position in a manner that maintains symmetry about an axis."@en ;
             rdfs:label "symmetricalRotationAct"@en .


###  http://www.semanticweb.org/CarterBenson/FutOnFutOn_00016
:FutOn_00016 rdf:type owl:Class ;
             rdfs:subClassOf :FutOn_00014 ;
             obo:IAO_0000115 "asymmetricalRotationAct in football is a rotationAct that describes a strategic movement or action in which players rotate and change position in a manner that does not maintain symmetry about an axis."@en ;
             rdfs:label "asymmetricalRotationAct"@en .


###  http://www.semanticweb.org/CarterBenson/FutOnFutOn_00017
:FutOn_00017 rdf:type owl:Class ;
             rdfs:subClassOf :FutOn_00013 ;
             obo:IAO_0000115 "onBallAct is an inPossessionAct that involves a player maintaining control over the ball duringmatchplay."@en ;
             rdfs:label "onBallAct"@en .


###  http://www.semanticweb.org/CarterBenson/FutOnFutOn_00018
:FutOn_00018 rdf:type owl:Class ;
             rdfs:subClassOf :FutOn_00017 ;
             obo:IAO_0000115 "shotAct is an onBallAct that is performed by a player when they attempt to propel the ball into the opponent's goal."@en ;
             rdfs:label "shotAct"@en .


###  http://www.semanticweb.org/CarterBenson/FutOnFutOn_00019
:FutOn_00019 rdf:type owl:Class ;
             rdfs:subClassOf :FutOn_00018 ;
             obo:IAO_0000115 "bendingShotAct is a shotAct that is performed by a player when they strike the ball in a way that causes it to curve in the air."@en ;
             rdfs:label "bendingShotAct"@en .


###  http://www.semanticweb.org/CarterBenson/FutOnFutOn_00020
:FutOn_00020 rdf:type owl:Class ;
             rdfs:subClassOf :FutOn_00018 ;
             obo:IAO_0000115 "bicycleShotAct is a shotAct that is performed by a player when they strike the ball in mid-air with a bicycle kick, a move where the player kicks the ball while performing a backflip."@en ;
             rdfs:label "bicycleShotAct"@en .


###  http://www.semanticweb.org/CarterBenson/FutOnFutOn_00021
:FutOn_00021 rdf:type owl:Class ;
             rdfs:subClassOf :FutOn_00018 ;
             obo:IAO_0000115 "chipShotAct is a shotAct that is performed by a player when they strike the ball in an upward trajectory with the aim of lobbing it over the goalkeeper and into the net."@en ;
             rdfs:label "chipShotAct"@en .


###  http://www.semanticweb.org/CarterBenson/FutOnFutOn_00022
:FutOn_00022 rdf:type owl:Class ;
             rdfs:subClassOf :FutOn_00018 ;
             obo:IAO_0000115 "headerShotAct is a shotAct that is performed by a player when they attempt to direct the ball into the opponent's goal by striking it with their head."@en ;
             rdfs:label "headerShotAct"@en .


###  http://www.semanticweb.org/CarterBenson/FutOnFutOn_00023
:FutOn_00023 rdf:type owl:Class ;
             rdfs:subClassOf :FutOn_00018 ;
             obo:IAO_0000115 "rabonaShotAct is a shotAct that is performed by a player when they wrap their kicking leg around the back of their standing leg to strike the ball."@en ;
             rdfs:label "rabonaShotAct"@en .


###  http://www.semanticweb.org/CarterBenson/FutOnFutOn_00024
:FutOn_00024 rdf:type owl:Class ;
             rdfs:subClassOf :FutOn_00018 ;
             obo:IAO_0000115 "standardShotAct is a shotAct that is performed by a player when they attempt to direct the ball into the opponent's goal by striking it with a standard kick, typically using the inside of the foot."@en ;
             rdfs:label "standardShotAct"@en .


###  http://www.semanticweb.org/CarterBenson/FutOnFutOn_00025
:FutOn_00025 rdf:type owl:Class ;
             rdfs:subClassOf :FutOn_00018 ;
             obo:IAO_0000115 "straightShotAct is a shotAct that is performed by a player when they strike the ball in a straight trajectory towards the opponent's goal."@en ;
             rdfs:label "straightShotAct"@en .


###  http://www.semanticweb.org/CarterBenson/FutOnFutOn_00026
:FutOn_00026 rdf:type owl:Class ;
             rdfs:subClassOf :FutOn_00018 ;
             obo:IAO_0000115 "volleyShotAct is a shotAct that is performed by a player when they strike the ball before it touches the ground, typically after a cross or a rebound."@en ;
             rdfs:label "volleyShotAct"@en .


###  http://www.semanticweb.org/CarterBenson/FutOnFutOn_00031
:FutOn_00031 rdf:type owl:Class ;
             rdfs:subClassOf :FutOn_00015 ;
             obo:IAO_0000115 "dribbleAct is an onBallAct that involves a player controlling the ball and moving it forward by repeatedly striking it with any part legal part of their body."@en ;
             rdfs:label "dribbleAct"@en .


###  http://www.semanticweb.org/CarterBenson/FutOnFutOn_00032
:FutOn_00032 rdf:type owl:Class ;
             rdfs:subClassOf :FutOn_00015 ;
             obo:IAO_0000115 "controlAct is an onBallAct that represents the action of a player successfully gaining possession of the ball from a pass or interception using any legal part of their body."@en ;
             rdfs:label "controlAct"@en .


###  http://www.semanticweb.org/CarterBenson/FutOnFutOn_00033
:FutOn_00033 rdf:type owl:Class ;
             rdfs:subClassOf :FutOn_00032 ;
             obo:IAO_0000115 "chestControl is a controlAct that describes the action of a player successfully gaining possession of the ball using their chest."@en ;
             rdfs:label "chestControl"@en .


###  http://www.semanticweb.org/CarterBenson/FutOnFutOn_00034
:FutOn_00034 rdf:type owl:Class ;
             rdfs:subClassOf :FutOn_00032 ;
             obo:IAO_0000115 "footControl is a controlAct that describes the action of a player successfully gaining possession of the ball using their foot."@en ;
             rdfs:label "footControl"@en .


###  http://www.semanticweb.org/CarterBenson/FutOnFutOn_00035
:FutOn_00035 rdf:type owl:Class ;
             rdfs:subClassOf :FutOn_00015 ;
             obo:IAO_0000115 "passAct is an onBallAct in which a player, who is in control of the ball, deliberately sends the ball to a teammate."@en ;
             rdfs:label "passAct"@en .


###  http://www.semanticweb.org/CarterBenson/FutOnFutOn_00036
:FutOn_00036 rdf:type owl:Class ;
             rdfs:subClassOf :FutOn_00035 ;
             obo:IAO_0000115 "crossAct is passAct that involves sending the ball across the field, usually from a wide position into the penalty area, aiming to reach a teammate."@en ;
             rdfs:label "crossAct"@en .


###  http://www.semanticweb.org/CarterBenson/FutOnFutOn_00037
:FutOn_00037 rdf:type owl:Class ;
             rdfs:subClassOf :FutOn_00035 ;
             obo:IAO_0000115 "giveAndGoAct is a passAct that consists of a player passing the ball to a teammate and then immediately moving forward to receive a return pass."@en ;
             rdfs:label "giveAndGoAct"@en .


###  http://www.semanticweb.org/CarterBenson/FutOnFutOn_00038
:FutOn_00038 rdf:type owl:Class ;
             rdfs:subClassOf :FutOn_00035 ;
             obo:IAO_0000115 "oneTouchPassAct is a passAct where the player passes the ball immediately upon receiving it, using just one touch."@en ;
             rdfs:label "oneTouchPassAct"@en .


###  http://www.semanticweb.org/CarterBenson/FutOnFutOn_00039
:FutOn_00039 rdf:type owl:Class ;
             rdfs:subClassOf :FutOn_00035 ;
             obo:IAO_0000115 "throughPassAct is a passAct in which a player sends the ball through the opponents' defensive line to a teammate, typically to create a scoring opportunity."@en ;
             rdfs:label "throughPassAct"@en .


###  http://www.semanticweb.org/CarterBenson/FutOnFutOn_00040
:FutOn_00040 rdf:type owl:Class ;
             rdfs:subClassOf :FutOn_00035 ;
             obo:IAO_0000115 "backHeelPassAct is a passAct that involves the player striking the ball with the back of their heel to pass it to a teammate, often employed to deceive the opposition."@en ;
             rdfs:label "backHeelPassAct"@en .


###  http://www.semanticweb.org/CarterBenson/FutOnFutOn_00041
:FutOn_00041 rdf:type owl:Class ;
             rdfs:subClassOf :FutOn_00035 ;
             obo:IAO_0000115 "outsideFootPass is a passAct where the player uses the outside of their foot to pass the ball, typically to curve it around an opponent or for a change in direction."@en ;
             rdfs:label "outsideFootPass"@en .


###  http://www.semanticweb.org/CarterBenson/FutOnFutOn_00042
:FutOn_00042 rdf:type owl:Class ;
             rdfs:subClassOf :FutOn_00035 ;
             obo:IAO_0000115 "pushPassAct is a passAct that involves the player using the inside of their foot to gently push the ball to a teammate, typically used for short, accurate passes."@en ;
             rdfs:label "pushPassAct"@en .


###  http://www.semanticweb.org/CarterBenson/FutOnFutOn_00044
:FutOn_00044 rdf:type owl:Class ;
             rdfs:subClassOf <http://www.ontologyrepository.com/CommonCoreOntologies/MeasurementInformationContentEntity> ;
             obo:IAO_0000115 "A measurementInformationContentEntity that quantifies or qualifies actions that take place in amatch."@en ;
             rdfs:label "MatchMeasurement"@en .


###  http://www.semanticweb.org/CarterBenson/FutOnFutOn_00045
:FutOn_00045 rdf:type owl:Class ;
             rdfs:subClassOf :FutOn_00044 ;
             obo:IAO_0000115 "AmatchMeasurement that represents a numeric or quantifiable property derived from amatch ormatch-related event."@en ;
             rdfs:label "MatchMeasurementQuantity"@en .


###  http://www.semanticweb.org/CarterBenson/FutOnFutOn_00046
:FutOn_00046 rdf:type owl:Class ;
             rdfs:subClassOf :FutOn_00045 ;
             obo:IAO_0000115 "AmatchMeasurementQuantity that quantifies the total number of successful tackles performed by a player or a team during amatch."@en ;
             rdfs:label "tackleTally"@en .


###  http://www.semanticweb.org/CarterBenson/FutOnFutOn_00047
:FutOn_00047 rdf:type owl:Class ;
             rdfs:subClassOf :FutOn_00045 ;
             obo:IAO_0000115 "AmatchMeasurementQuantity that quantifies the total number of successful interceptions performed by a player or a team during amatch."@en ;
             rdfs:label "interceptionTally"@en .


###  http://www.semanticweb.org/CarterBenson/FutOnFutOn_00048
:FutOn_00048 rdf:type owl:Class ;
             rdfs:subClassOf :FutOn_00045 ;
             obo:IAO_0000115 "AmatchMeasurementQuantity that quantifies the total number of successful goals scored by a player or a team during amatch."@en ;
             rdfs:label "goalTally"@en .


###  http://www.semanticweb.org/CarterBenson/FutOnFutOn_00049
:FutOn_00049 rdf:type owl:Class ;
             rdfs:subClassOf :FutOn_00045 ;
             obo:IAO_0000115 "AmatchMeasurementQuantity that specifically quantifies the number of shots taken or made during amatch."@en ;
             rdfs:label "shotTally"@en .


###  http://www.semanticweb.org/CarterBenson/FutOnFutOn_00050
:FutOn_00050 rdf:type owl:Class ;
             rdfs:subClassOf :FutOn_00049 ;
             obo:IAO_0000115 "A shotTally that quantifies the total number of shots taken or made by an entire team during amatch."@en ;
             rdfs:label "teamShotTally"@en .


###  http://www.semanticweb.org/CarterBenson/FutOnFutOn_00051
:FutOn_00051 rdf:type owl:Class ;
             rdfs:subClassOf :FutOn_00049 ;
             obo:IAO_0000115 "A shotTally that quantifies the total number of shots taken or made by an individual player during amatch."@en ;
             rdfs:label "playerShotTally"@en .


###  http://www.semanticweb.org/CarterBenson/FutOnFutOn_00052
:FutOn_00052 rdf:type owl:Class ;
             rdfs:subClassOf :FutOn_00045 ;
             obo:IAO_0000115 "AmatchMeasurementQuantity that specifically quantifies the total number of passes made during amatch."@en ;
             rdfs:label "passTally"@en .


###  http://www.semanticweb.org/CarterBenson/FutOnFutOn_00053
:FutOn_00053 rdf:type owl:Class ;
             rdfs:subClassOf :FutOn_00052 ;
             obo:IAO_0000115 "A passTally that quantifies the total number of passes made by an individual player during amatch."@en ;
             rdfs:label "playerPassTally"@en .


###  http://www.semanticweb.org/CarterBenson/FutOnFutOn_00054
:FutOn_00054 rdf:type owl:Class ;
             rdfs:subClassOf :FutOn_00052 ;
             obo:IAO_0000115 "A passTally that quantifies the total number of passes made by an entire team during amatch ormatch-related event."@en ;
             rdfs:label "teamPassTally"@en .


###  http://www.semanticweb.org/CarterBenson/FutOnFutOn_00055
:FutOn_00055 rdf:type owl:Class ;
             rdfs:subClassOf :FutOn_00045 ;
             obo:IAO_0000115 "AmatchMeasurementQuantity that specifically represents the output of an xGAlgorithm, quantifying the probability of a shot resulting in a goal in amatch."@en ;
             rdfs:label "xGValue"@en .


###  http://www.semanticweb.org/CarterBenson/FutOnFutOn_00056
:FutOn_00056 rdf:type owl:Class ;
             rdfs:subClassOf :FutOn_00055 ;
             obo:IAO_0000115 "An xGValue that represents the xGValue for an individual player."@en ;
             rdfs:label "xGValuePlayer"@en .


###  http://www.semanticweb.org/CarterBenson/FutOnFutOn_00057
:FutOn_00057 rdf:type owl:Class ;
             rdfs:subClassOf :FutOn_00055 ;
             obo:IAO_0000115 "An xGValue that represents the total Expected Goals (xG) value for a team in amatch, calculated as the sum of the xGValues for all individual players on the team."@en ;
             rdfs:label "xGValueTeam"@en .


###  http://www.semanticweb.org/CarterBenson/FutOnFutOn_00058
:FutOn_00058 rdf:type owl:Class ;
             rdfs:subClassOf :FutOn_00045 ;
             obo:IAO_0000115 "AmatchMeasurementQuantity that quantifies the likelihood that a given pass will lead to a shot and subsequently a goal, based on various factors such as the type of pass, its origin and destination points, and the historical data."@en ;
             rdfs:label "xAValue"@en .


###  http://www.semanticweb.org/CarterBenson/FutOnFutOn_00059
:FutOn_00059 rdf:type owl:Class ;
             rdfs:subClassOf :FutOn_00045 ;
             obo:IAO_0000115 "AmatchMeasurementQuantity that quantifies the predicted number of points a team is expected to earn from amatch based on the team's total xGValue, which is calculated from individual shot xGValues during thematch."@en ;
             rdfs:label "xPValue"@en .


###  http://www.semanticweb.org/CarterBenson/FutOnFutOn_00060
:FutOn_00060 rdf:type owl:Class ;
             rdfs:subClassOf :FutOn_00044 ;
             obo:IAO_0000115 "AmatchMeasurement that specifically represents a qualitative or descriptive attribute associated with amatch."@en ;
             rdfs:label "MatchMeasurementQuality"@en .


###  http://www.semanticweb.org/CarterBenson/FutOnFutOn_00061
:FutOn_00061 rdf:type owl:Class ;
             rdfs:subClassOf :FutOn_00060 ;
             obo:IAO_0000115 "AmatchMeasurementQuality that involves a comprehensive evaluation ofmatch dynamics, player performance, and team strategy, based on the xG values and potentially including other qualitative assessments."@en ;
             rdfs:label "xGAnalysis"@en .


###  http://www.semanticweb.org/CarterBenson/FutOnFutOn_00062
:FutOn_00062 rdf:type owl:Class ;
             rdfs:subClassOf :FutOn_00060 ;
             obo:IAO_0000115 "AmatchMeasurementQuality that assesses the quality of an individual player's performance during amatch ormatch-related event, often on a scale (e.g., 1-10)."@en ;
             rdfs:label "playerPerformanceRating"@en .


###  http://www.semanticweb.org/CarterBenson/FutOnFutOn_00063
:FutOn_00063 rdf:type owl:Class ;
             rdfs:subClassOf :FutOn_00060 ;
             obo:IAO_0000115 "AmatchMeasurementQuality that identifies a specific phase or period of amatch ormatch-related event (e.g., first half, second half, overtime)."@en ;
             rdfs:label "MatchPhaseIdentification"@en .


###  http://www.semanticweb.org/CarterBenson/FutOnFutOn_00064
:FutOn_00064 rdf:type owl:Class ;
             rdfs:subClassOf :FutOn_00060 ;
             obo:IAO_0000115 "AmatchMeasurementQuality that represents an evaluation of the effectiveness of a player's markingAct in amatch. This may be quantified by a number of factors, including but not limited to the number of times the marked opponent was dispossessed, the number of unsuccessful plays made by the marked opponent, the marked opponent's influence on thematch relative to their average performance, and the outcome of thematch."@en ;
             rdfs:label "markingQuality"@en .


###  http://www.semanticweb.org/CarterBenson/FutOnFutOn_00065
:FutOn_00065 rdf:type owl:Class ;
             rdfs:subClassOf <http://www.ontologyrepository.com/CommonCoreOntologies/Algorithm> ;
             obo:IAO_0000115 "An Algorithm that is specifically designed to take as input data about a shot, such as its distance, angle, context (e.g., open play, set-piece, etc.), and potentially other factors, and output an xGValue."@en ;
             rdfs:label "xGAlgorithm"@en .


###  http://www.semanticweb.org/CarterBenson/FutOnFutOn_00066
:FutOn_00066 rdf:type owl:Class ;
             rdfs:subClassOf <http://www.ontologyrepository.com/CommonCoreOntologies/Algorithm> ;
             obo:IAO_0000115 "An Algorithm that is specifically designed to take as input data about a pass, such as its type, origin and destination points, and other contextual factors, and output an xAValue, which quantifies the likelihood that the given pass will lead to a shot and subsequently a goal."@en ;
             rdfs:label "xAAlgorithm"@en .


###  http://www.semanticweb.org/CarterBenson/FutOnFutOn_00068
:FutOn_00068 rdf:type owl:Class ;
             rdfs:subClassOf <http://www.ontologyrepository.com/CommonCoreOntologies/PredictiveInformationContentEntity> ;
             obo:IAO_0000115 "A PredictiveInformationContentEntity used to predict the outcome of a footballmatch or series ofmatches, based on the sum of Expected Goals (xG) values of a team. It predicts the number of points a team is likely to earn from thematch(es)."@en ;
             rdfs:label "xPForGamblers"@en .


###  http://www.semanticweb.org/CarterBenson/FutOnFutOn_00069
:FutOn_00069 rdf:type owl:Class ;
             rdfs:subClassOf <http://www.ontologyrepository.com/CommonCoreOntologies/PredictiveInformationContentEntity> ;
             obo:IAO_0000115 "A PredictiveInformationContentEntity used to predict the outcome of a footballmatch, based on the quantity and quality of shots taken by a team or player. It quantifies the probability of each shot resulting in a goal, considering various factors like distance from the goal, angle to the goal,match context, and historical data."@en ;
             rdfs:label "xGforGamblers"@en .


###  http://www.semanticweb.org/CarterBenson/FutOnFutOn_00070
:FutOn_00070 rdf:type owl:Class ;
             rdfs:subClassOf <http://www.ontologyrepository.com/CommonCoreOntologies/Ideology> ;
             obo:IAO_0000115 "An Ideology that represents the guiding principles, values, and strategic approach a football club adopts and adheres to in its operations, including player development,match strategy, and club management."@en ;
             rdfs:label "clubPhilosophy"@en .


###  http://www.semanticweb.org/CarterBenson/FutOnFutOn_00071
:FutOn_00071 rdf:type owl:Class ;
             rdfs:subClassOf :FutOn_00070 ;
             obo:IAO_0000115 "A clubPhilosophy that emphasizes the use of Expected Goals (xG) metrics in various aspects of the football club's operations and strategy, including player performance analysis, team strategy, talent scouting, and player training."@en ;
             rdfs:label "xGPhilosophy"@en .


###  http://www.semanticweb.org/CarterBenson/FutOnFutOn_00074
:FutOn_00074 rdf:type owl:Class ;
             rdfs:subClassOf :FutOn_00002 ;
             obo:IAO_0000115 "A refereeAct that represents the action of making decisions on rule infractions during a game."@en ;
             rdfs:label "decisionAct"@en .


###  http://www.semanticweb.org/CarterBenson/FutOnFutOn_00075
:FutOn_00075 rdf:type owl:Class ;
             rdfs:subClassOf :FutOn_00074 ;
             obo:IAO_0000115 "A decisionAct that represents the referee's action of making a decision related to fouls committed by players during a game."@en ;
             rdfs:label "foulDecisionAct"@en .


###  http://www.semanticweb.org/CarterBenson/FutOnFutOn_00076
:FutOn_00076 rdf:type owl:Class ;
             rdfs:subClassOf :FutOn_00075 ;
             obo:IAO_0000115 "A foulDecisionAct that signifies the referee's action of making a decision regarding a suspected handball offense."@en ;
             rdfs:label "handballCall"@en .


###  http://www.semanticweb.org/CarterBenson/FutOnFutOn_00077
:FutOn_00077 rdf:type owl:Class ;
             rdfs:subClassOf :FutOn_00075 ;
             obo:IAO_0000115 "A foulDecisionAct that signifies the referee's action of deciding on potential offside situations in a game."@en ;
             rdfs:label "offsideDecisionAct"@en .


###  http://www.semanticweb.org/CarterBenson/FutOnFutOn_00078
:FutOn_00078 rdf:type owl:Class ;
             rdfs:subClassOf :FutOn_00075 ;
             obo:IAO_0000115 "A foulDecisionAct that encompasses the referee's action of deciding to issue a yellow or red card to a player."@en ;
             rdfs:label "cardDecisionAct"@en .


###  http://www.semanticweb.org/CarterBenson/FutOnFutOn_00079
:FutOn_00079 rdf:type owl:Class ;
             rdfs:subClassOf :FutOn_00078 ;
             obo:IAO_0000115 "A cardDecisionAct that represents the referee's action of deciding to issue a yellow card to a player for a particular misconduct."@en ;
             rdfs:label "yellowCardDecisionAct"@en .


###  http://www.semanticweb.org/CarterBenson/FutOnFutOn_00080
:FutOn_00080 rdf:type owl:Class ;
             rdfs:subClassOf :FutOn_00078 ;
             obo:IAO_0000115 "A cardDecisionAct that signifies the referee's action of deciding to issue a red card, either for a severe infraction or for a second yellow card offense in the same game."@en ;
             rdfs:label "redCardDecisionAct"@en .


###  http://www.semanticweb.org/CarterBenson/FutOnFutOn_00081
:FutOn_00081 rdf:type owl:Class ;
             rdfs:subClassOf :FutOn_00002 ;
             obo:IAO_0000115 "A refereeAct that denotes the action of starting and stopping play during a game."@en ;
             rdfs:label "startingStoppingAct"@en .


###  http://www.semanticweb.org/CarterBenson/FutOnFutOn_00082
:FutOn_00082 rdf:type owl:Class ;
             rdfs:subClassOf :FutOn_00081 ;
             obo:IAO_0000115 "A startingStoppingAct that signifies the referee's action of restarting the game after a foul has been addressed."@en ;
             rdfs:label "foulRestartAct"@en .


###  http://www.semanticweb.org/CarterBenson/FutOnFutOn_00083
:FutOn_00083 rdf:type owl:Class ;
             rdfs:subClassOf :FutOn_00081 ;
             obo:IAO_0000115 "A startingStoppingAct that represents the referee's action of stopping the game due to a foul."@en ;
             rdfs:label "foulStopAct"@en .


###  http://www.semanticweb.org/CarterBenson/FutOnFutOn_00084
:FutOn_00084 rdf:type owl:Class ;
             rdfs:subClassOf :FutOn_00081 ;
             obo:IAO_0000115 "A startingStoppingAct that represents the referee's action of initiating the start of a game."@en ;
             rdfs:label "gameStartAct"@en .


###  http://www.semanticweb.org/CarterBenson/FutOnFutOn_00085
:FutOn_00085 rdf:type owl:Class ;
             rdfs:subClassOf :FutOn_00081 ;
             obo:IAO_0000115 "A startingStoppingAct that signifies the referee's action of calling the end of a game."@en ;
             rdfs:label "gameStopAct"@en .


###  http://www.semanticweb.org/CarterBenson/FutOnFutOn_00086
:FutOn_00086 rdf:type owl:Class ;
             rdfs:subClassOf :FutOn_00081 ;
             obo:IAO_0000115 "A startingStoppingAct that denotes the referee's action of initiating the start of the second half of a game."@en ;
             rdfs:label "halfTimeStartAct"@en .


###  http://www.semanticweb.org/CarterBenson/FutOnFutOn_00087
:FutOn_00087 rdf:type owl:Class ;
             rdfs:subClassOf :FutOn_00081 ;
             obo:IAO_0000115 "A startingStoppingAct that embodies the referee's action of declaring the end of the first half of a game."@en ;
             rdfs:label "halfTimeStopAct"@en .


###  http://www.semanticweb.org/CarterBenson/FutOnFutOn_00088
:FutOn_00088 rdf:type owl:Class ;
             rdfs:subClassOf :FutOn_00002 ;
             obo:IAO_0000115 "A refereeAct that encompasses all actions related to keeping track of time during a game."@en ;
             rdfs:label "timeKeepingAct"@en .


###  http://www.semanticweb.org/CarterBenson/FutOnFutOn_00089
:FutOn_00089 rdf:type owl:Class ;
             rdfs:subClassOf :FutOn_00088 ;
             obo:IAO_0000115 "A timeKeepingAct that represents the referee's action of monitoring the overall game clock."@en ;
             rdfs:label "gameClockMonitoringAct"@en .


###  http://www.semanticweb.org/CarterBenson/FutOnFutOn_00090
:FutOn_00090 rdf:type owl:Class ;
             rdfs:subClassOf :FutOn_00088 ;
             obo:IAO_0000115 "A timeKeepingAct that denotes the referee's action of adding or subtracting stoppage time due to delays like injuries or interruptions."@en ;
             rdfs:label "stoppageTimeAdjustmentAct"@en .


###  http://www.semanticweb.org/CarterBenson/FutOnFutOn_00091
:FutOn_00091 rdf:type owl:Class ;
             rdfs:subClassOf :FutOn_00088 ;
             obo:IAO_0000115 "A timeKeepingAct that signifies the referee's action of keeping track of the time elapsed in each half of the game."@en ;
             rdfs:label "halfTimeMonitoringAct"@en .


###  http://www.semanticweb.org/CarterBenson/FutOnFutOn_00092
:FutOn_00092 rdf:type owl:Class ;
             rdfs:subClassOf :FutOn_00088 ;
             obo:IAO_0000115 "A timeKeepingAct that embodies the referee's action of keeping track of additional time periods in games that may go into extra time or overtime."@en ;
             rdfs:label "extraTimeMonitoringAct"@en .


###  http://www.semanticweb.org/CarterBenson/FutOnFutOn_00093
:FutOn_00093 rdf:type owl:Class ;
             rdfs:subClassOf :FutOn_00002 ;
             obo:IAO_0000115 "A refereeAct that signifies actions aimed at enforcing the rules of the game and ensuring fair play."@en ;
             rdfs:label "fairPlayEnforcementAct"@en .


###  http://www.semanticweb.org/CarterBenson/FutOnFutOn_00094
:FutOn_00094 rdf:type owl:Class ;
             rdfs:subClassOf :FutOn_00093 ;
             obo:IAO_0000115 "A fairPlayEnforcementAct that signifies the referee's action of penalizing player misconducts, in order to maintain fair play."@en ;
             rdfs:label "misconductPenalizingAct"@en .


###  http://www.semanticweb.org/CarterBenson/FutOnFutOn_00095
:FutOn_00095 rdf:type owl:Class ;
             rdfs:subClassOf :FutOn_00093 ;
             obo:IAO_0000115 "A fairPlayEnforcementAct that denotes the referee's action of advocating for fair play, such as by managing player behavior, mediating disputes, or addressing unsportsmanlike conduct."@en ;
             rdfs:label "fairPlayAdvocacyAct"@en .


###  http://www.semanticweb.org/CarterBenson/FutOnFutOn_00096
:FutOn_00096 rdf:type owl:Class ;
             rdfs:subClassOf :FutOn_00093 ;
             obo:IAO_0000115 "A fairPlayEnforcementAct that embodies the referee's action of controlling the overall game situation to ensure fair play, such as by managing player emotions, defusing tense situations, and so on."@en ;
             rdfs:label "gameControlAct"@en .


###  http://www.semanticweb.org/CarterBenson/FutOnFutOn_00097
:FutOn_00097 rdf:type owl:Class ;
             rdfs:subClassOf :FutOn_00098 ;
             obo:IAO_0000115 "A managerAct that represents the action of selecting which players will start the game or be on the bench."@en ;
             rdfs:label "playerSelectionAct"@en .


###  http://www.semanticweb.org/CarterBenson/FutOnFutOn_00098
:FutOn_00098 rdf:type owl:Class ;
             rdfs:subClassOf :FutOn_00003 ;
             obo:IAO_0000115 "A managerAct that signifies the manager's action of planning game strategies, deciding formations, and preparing tactical approaches."@en ;
             rdfs:label "strategyPlanningAct"@en .


###  http://www.semanticweb.org/CarterBenson/FutOnFutOn_00099
:FutOn_00099 rdf:type owl:Class ;
             rdfs:subClassOf :FutOn_00003 ;
             obo:IAO_0000115 "A managerAct that denotes the manager's action of deciding when and which player should be substituted during a game."@en ;
             rdfs:label "substitutionAct"@en .


###  http://www.semanticweb.org/CarterBenson/FutOnFutOn_00100
:FutOn_00100 rdf:type owl:Class ;
             rdfs:subClassOf :FutOn_00099 ;
             obo:IAO_0000115 "A substitutionAct that represents the manager's action of substituting a player due to injury."@en ;
             rdfs:label "injurySubstitutionAct"@en .


###  http://www.semanticweb.org/CarterBenson/FutOnFutOn_00101
:FutOn_00101 rdf:type owl:Class ;
             rdfs:subClassOf :FutOn_00099 ;
             obo:IAO_0000115 "A substitutionAct that signifies the manager's action of substituting a player to implement a new tactical approach or to strengthen a particular area of the team."@en ;
             rdfs:label "tacticalSubstitutionAct"@en .


###  http://www.semanticweb.org/CarterBenson/FutOnFutOn_00102
:FutOn_00102 rdf:type owl:Class ;
             rdfs:subClassOf :FutOn_00099 ;
             obo:IAO_0000115 "A substitutionAct that denotes the manager's action of substituting a player due to disciplinary issues, such as to prevent a player at risk of receiving a red card from being sent off."@en ;
             rdfs:label "disciplinarySubstitutionAct"@en .


###  http://www.semanticweb.org/CarterBenson/FutOnFutOn_00103
:FutOn_00103 rdf:type owl:Class ;
             rdfs:subClassOf :FutOn_00099 ;
             obo:IAO_0000115 "A substitutionAct that represents the manager's action of substituting a player who is tired or not performing optimally due to fatigue."@en ;
             rdfs:label "fatigueSubstitutionAct"@en .


###  http://www.semanticweb.org/CarterBenson/FutOnFutOn_00104
:FutOn_00104 rdf:type owl:Class ;
             rdfs:subClassOf :FutOn_00099 ;
             obo:IAO_0000115 "A substitutionAct that embodies the manager's action of substituting a player in order to waste time, usually towards the end of the game when the team is leading."@en ;
             rdfs:label "timeWastingSubstitutionAct"@en .


###  http://www.semanticweb.org/CarterBenson/FutOnFutOn_00105
:FutOn_00105 rdf:type owl:Class ;
             rdfs:subClassOf :FutOn_00003 ;
             obo:IAO_0000115 "A managerAct that embodies the manager's action of communicating instructions, feedback, or motivational speeches to players."@en ;
             rdfs:label "communicationAct"@en .


###  http://www.semanticweb.org/CarterBenson/FutOnFutOn_00106
:FutOn_00106 rdf:type owl:Class ;
             rdfs:subClassOf :FutOn_00003 ;
             obo:IAO_0000115 "A managerAct that represents the action of a manager analyzing the strategies, strengths, and weaknesses of opponent teams."@en ;
             rdfs:label "opponentAnalysisAct"@en .


###  http://www.semanticweb.org/CarterBenson/FutOnFutOn_00107
:FutOn_00107 rdf:type owl:Class ;
             rdfs:subClassOf :FutOn_00098 ;
             obo:IAO_0000115 "A strategyPlanningAct that represents the manager's action of selecting the team's formation for a game."@en ;
             rdfs:label "formationSelectionAct"@en .


###  http://www.semanticweb.org/CarterBenson/FutOnFutOn_00108
:FutOn_00108 rdf:type owl:Class ;
             rdfs:subClassOf :FutOn_00098 ;
             obo:IAO_0000115 "A strategyPlanningAct that signifies the manager's action of preparing set piece strategies, such as free kicks, corners, or penalty kicks."@en ;
             rdfs:label "setPiecePreparationAct"@en .


###  http://www.semanticweb.org/CarterBenson/FutOnFutOn_00109
:FutOn_00109 rdf:type owl:Class ;
             rdfs:subClassOf :FutOn_00106 ;
             obo:IAO_0000115 "An opponentAnalysisAct that represents the manager's action of analyzing the strategies, strengths, and weaknesses of specific opponent teams."@en ;
             rdfs:label "oppositionAnalysisAct"@en .


###  http://www.semanticweb.org/CarterBenson/FutOnFutOn_00110
:FutOn_00110 rdf:type owl:Class ;
             rdfs:subClassOf :FutOn_00106 ;
             obo:IAO_0000115 "An opponentAnalysisAct that signifies the manager's action of assessing individual players of the opponent team, their strengths, weaknesses, and playing styles."@en ;
             rdfs:label "playerAssessmentAct"@en .


###  http://www.semanticweb.org/CarterBenson/FutOnFutOn_00112
:FutOn_00112 rdf:type owl:Class ;
             rdfs:subClassOf :FutOn_00013 ;
             obo:IAO_0000115 "An offBallAct that represents actions performed by a player when not in possession of the ball during a game."@en ;
             rdfs:label "offBallAct"@en .


###  http://www.semanticweb.org/CarterBenson/FutOnFutOn_00134
:FutOn_00134 rdf:type owl:Class ;
             rdfs:subClassOf :FutOnn_00121 ;
             obo:IAO_0000115 "A playerPosition in which a player is responsible for guarding the team's goal and preventing the opposing team from scoring. This is the only position allowed to handle the ball within the penalty area."@en ;
             rdfs:label "goalkeeper"@en .


###  http://www.semanticweb.org/CarterBenson/FutOnFutOn_00135
:FutOn_00135 rdf:type owl:Class ;
             rdfs:subClassOf :FutOnn_00121 ;
             obo:IAO_0000115 "A playerPosition that involves a player primarily focusing on preventing the opposing team from scoring. Subclasses could include center-back, full-back, wing-back, and sweeper."@en ;
             rdfs:label "defender"@en .


###  http://www.semanticweb.org/CarterBenson/FutOnFutOn_00136
:FutOn_00136 rdf:type owl:Class ;
             rdfs:subClassOf :FutOn_00135 ;
             obo:IAO_0000115 "A defender where the player occupies a central position in defense, typically focusing on intercepting passes, blocking shots, and marking opposing forwards."@en ;
             rdfs:label "centerBack"@en .


###  http://www.semanticweb.org/CarterBenson/FutOnFutOn_00137
:FutOn_00137 rdf:type owl:Class ;
             rdfs:subClassOf :FutOn_00135 ;
             obo:IAO_0000115 "A defender where the player occupies the flanks of the defense, often contributing to both defensive tasks and attacking plays along the wings."@en ;
             rdfs:label "fullBack"@en .


###  http://www.semanticweb.org/CarterBenson/FutOnFutOn_00138
:FutOn_00138 rdf:type owl:Class ;
             rdfs:subClassOf :FutOn_00137 ;
             obo:IAO_0000115 "A fullBack often used in formations that utilize three center-backs. These players patrol wide areas of the pitch, supporting both defensive and offensive tasks."@en ;
             rdfs:label "wingBack"@en .


###  http://www.semanticweb.org/CarterBenson/FutOnFutOn_00139
:FutOn_00139 rdf:type owl:Class ;
             rdfs:subClassOf :FutOn_00135 ;
             obo:IAO_0000115 "A defender often positioned behind the line of defenders, focusing on clearing the ball from the defensive zone and covering defensive gaps."@en ;
             rdfs:label "sweeper"@en .


###  http://www.semanticweb.org/CarterBenson/FutOnFutOn_00140
:FutOn_00140 rdf:type owl:Class ;
             rdfs:subClassOf :FutOnn_00121 ;
             obo:IAO_0000115 "A player that involves a player operating in the area of the field between the defense and the forwards, often involved in both attacking and defensive duties. Subclasses could include central midfielder, attacking midfielder, defensive midfielder, and wide midfielder."@en ;
             rdfs:label "midfielder"@en .


###  http://www.semanticweb.org/CarterBenson/FutOnFutOn_00141
:FutOn_00141 rdf:type owl:Class ;
             rdfs:subClassOf :FutOn_00140 ;
             obo:IAO_0000115 "A midfielder where the player is often involved in both attacking and defensive duties, distributing the ball, and maintaining possession."@en ;
             rdfs:label "centralMidfielder"@en .


###  http://www.semanticweb.org/CarterBenson/FutOnFutOn_00142
:FutOn_00142 rdf:type owl:Class ;
             rdfs:subClassOf :FutOn_00140 ;
             obo:IAO_0000115 "A midfielder where the player is positioned closer to the forwards and focuses on creating scoring opportunities."@en ;
             rdfs:label "attackingMidfielder"@en .


###  http://www.semanticweb.org/CarterBenson/FutOnFutOn_00143
:FutOn_00143 rdf:type owl:Class ;
             rdfs:subClassOf :FutOn_00140 ;
             obo:IAO_0000115 "A midfielder where the player is positioned closer to the defense and focuses on shielding the defensive line and disrupting opposing attacks."@en ;
             rdfs:label "defensiveMidfielder"@en .


###  http://www.semanticweb.org/CarterBenson/FutOnFutOn_00144
:FutOn_00144 rdf:type owl:Class ;
             rdfs:subClassOf :FutOn_00140 ;
             obo:IAO_0000115 "A midfielder where the player occupies the flanks of the field, often contributing to both defensive tasks and attacking plays along the wings."@en ;
             rdfs:label "wideMidfielder"@en .


###  http://www.semanticweb.org/CarterBenson/FutOnFutOn_00145
:FutOn_00145 rdf:type owl:Class ;
             rdfs:subClassOf :FutOn_00144 ;
             obo:IAO_0000115 "A wideMidfielder in which a player operates primarily on the left side of the field."@en ;
             rdfs:label "leftMidfielder"@en .


###  http://www.semanticweb.org/CarterBenson/FutOnFutOn_00146
:FutOn_00146 rdf:type owl:Class ;
             rdfs:subClassOf :FutOn_00134 ;
             obo:IAO_0000115 "A playerPosition that involves a player primarily focusing on scoring goals and creating attacking opportunities."@en ;
             rdfs:label "forward"@en .


###  http://www.semanticweb.org/CarterBenson/FutOnFutOn_00147
:FutOn_00147 rdf:type owl:Class ;
             rdfs:subClassOf :FutOn_00146 ;
             obo:IAO_0000115 "A forward where the player leads the attack by positioning centrally, often the primary target for scoring opportunities."@en ;
             rdfs:label "centerForward"@en .


###  http://www.semanticweb.org/CarterBenson/FutOnFutOn_00148
:FutOn_00148 rdf:type owl:Class ;
             rdfs:subClassOf :FutOn_00146 ;
             obo:IAO_0000115 "A forward where the player supports the main striker, often dropping deeper into the midfield to receive the ball, turn, and run at the defense."@en ;
             rdfs:label "secondStriker"@en .


###  http://www.semanticweb.org/CarterBenson/FutOnFutOn_00149
:FutOn_00149 rdf:type owl:Class ;
             rdfs:subClassOf :FutOn_00146 ;
             obo:IAO_0000115 "A forward where the player is positioned on the wide parts of the pitch, often focusing on delivering crosses into the penalty area."@en ;
             rdfs:label "winger"@en .


###  http://www.semanticweb.org/CarterBenson/FutOnFutOn_00150
:FutOn_00150 rdf:type owl:Class ;
             rdfs:subClassOf :FutOn_00146 ;
             obo:IAO_0000115 "A forward where the player, while nominally a striker, drops deep into midfield to disrupt defensive lines and create space for teammates."@en ;
             rdfs:label "falseNine"@en .


###  http://www.semanticweb.org/CarterBenson/FutOnFutOn_00151
:FutOn_00151 rdf:type owl:Class ;
             rdfs:subClassOf :FutOn_00004 ;
             obo:IAO_0000115 "A playerAct that involves actions performed by the players actively participating on the soccer pitch during the match."@en ;
             rdfs:label "selectedPlayerAct"@en .


###  http://www.semanticweb.org/CarterBenson/FutOnFutOnn_00121
:FutOnn_00121 rdf:type owl:Class ;
              rdfs:subClassOf <http://www.ontologyrepository.com/CommonCoreOntologies/OccupationRole> ;
              obo:IAO_0000115 "an occupationRole that involves a person actively participating in the game of football under the rules and structures established by a governing body."@en ;
              rdfs:label "football Player"@en .


###  http://www.semanticweb.org/CarterBenson/FutOnFutOn:00001
<http://www.semanticweb.org/CarterBenson/FutOnFutOn:00001> rdf:type owl:Class ;
                                                           rdfs:subClassOf <http://www.ontologyrepository.com/CommonCoreOntologies/IntentionalAct> ;
                                                           obo:IAO_0000115 "an intentionalAct that represents any action deliberately performed by an individual during amatch."@en ;
                                                           rdfs:comment "These actions can range from playing actions (like shooting, passing, or tackling) performed by players, to strategic decisions and instructions given by coaches, to rulings and decisions made by referees."@en ;
                                                           rdfs:label "intentionalMatchAct"@en .


###  Generated by the OWL API (version 4.5.9.2019-02-01T07:24:44Z) https://github.com/owlcs/owlapi
