@prefix : <http://www.semanticweb.org/carte/ontologies/2023/6/untitled-ontology-63#> .
@prefix owl: <http://www.w3.org/2002/07/owl#> .
@prefix rdf: <http://www.w3.org/1999/02/22-rdf-syntax-ns#> .
@prefix xml: <http://www.w3.org/XML/1998/namespace> .
@prefix xsd: <http://www.w3.org/2001/XMLSchema#> .
@prefix rdfs: <http://www.w3.org/2000/01/rdf-schema#> .
@base <http://www.semanticweb.org/CarterBenson/FutOn/Prov/Definitions> .

<http://www.semanticweb.org/CarterBenson/FutOn/Prov/Definitions> rdf:type owl:Ontology .

#################################################################
#    Annotation properties
#################################################################



###  http://purl.obolibrary.org/obo/IAO_0000115
<http://purl.obolibrary.org/obo/IAO_0000115> rdf:type owl:AnnotationProperty ;
                                            rdfs:label "defintion"@en .


#################################################################
#    Classes
#################################################################

###  IAO:0000115/IntentionalAct
<IAO:0000115/IntentionalAct> rdf:type owl:Class .


###  IAO:0000115/measurementInformationContentEntityFutOn10002
<IAO:0000115/measurementInformationContentEntityFutOn10002> rdf:type owl:Class ;
                                                            rdfs:label "MeasurementInformationContentEntity" .


###  IAO:0000115/AlgorithmFutOn:10000FutOn:10000
<IAO:0000115/AlgorithmFutOn:10000FutOn:10000> rdf:type owl:Class ;
                                              rdfs:label "Algorithm" .


###  IAO:0000115/IdeologyFutOn:10001
<IAO:0000115/IdeologyFutOn:10001> rdf:type owl:Class ;
                                  rdfs:label "Ideology" .


###  IAO:0000115/PredictiveInformationContentEntityFutOn:10003
<IAO:0000115/PredictiveInformationContentEntityFutOn:10003> rdf:type owl:Class ;
                                                            rdfs:label "PredictiveInformationContentEntity" .


###  http://purl.obolibrary.org/obo/FutOn_00002
<http://purl.obolibrary.org/obo/FutOn_00002> rdf:type owl:Class ;
                                             rdfs:subClassOf <http://www.semanticweb.org/carte/ontologies/2023/6/untitled-ontology-63/FutOn:00001> ;
                                             <http://purl.obolibrary.org/obo/IAO_0000115> "an intentionalGameAct that represents any action deliberately performed by a referee during a game. These actions can include making decisions on rule infractions, starting and stopping play, time-keeping, and any other actions aimed at enforcing the rules of the game and ensuring fair play."@en ;
                                             rdfs:label "refereeAct"@en .


###  http://purl.obolibrary.org/obo/FutOn_00003
<http://purl.obolibrary.org/obo/FutOn_00003> rdf:type owl:Class ;
                                             rdfs:subClassOf <http://www.semanticweb.org/carte/ontologies/2023/6/untitled-ontology-63/FutOn:00001> ;
                                             <http://purl.obolibrary.org/obo/IAO_0000115> "an intentionalGameAct that represents any action deliberately performed by a team's manager or coach during a game. These actions can include strategic decisions, substitutions, tactical instructions, and any other actions aimed at guiding the team's play and strategy."@en ;
                                             rdfs:label "managerAct"@en .


###  http://purl.obolibrary.org/obo/FutOn_00004
<http://purl.obolibrary.org/obo/FutOn_00004> rdf:type owl:Class ;
                                             rdfs:subClassOf <http://www.semanticweb.org/carte/ontologies/2023/6/untitled-ontology-63/FutOn:00001> ;
                                             <http://purl.obolibrary.org/obo/IAO_0000115> "an intentionalGameAct that represents any action performed intentionally by a player during a game."@en ;
                                             rdfs:label "playerAct"@en .


###  http://purl.obolibrary.org/obo/FutOn_00005
<http://purl.obolibrary.org/obo/FutOn_00005> rdf:type owl:Class ;
                                             rdfs:subClassOf <http://purl.obolibrary.org/obo/FutOn_00004> ;
                                             <http://purl.obolibrary.org/obo/IAO_0000115> "is a playerAct that involves actions taken by a player when their team does not have control of the ball."@en ;
                                             rdfs:label "outOfPossessionAct"@en .


###  http://purl.obolibrary.org/obo/FutOn_00006
<http://purl.obolibrary.org/obo/FutOn_00006> rdf:type owl:Class ;
                                             rdfs:subClassOf <http://purl.obolibrary.org/obo/FutOn_00005> ;
                                             <http://purl.obolibrary.org/obo/IAO_0000115> "an outOfPossessionAct, that involves a player positioning themselves close to a specific opposing player with the intent of limiting their influence on the game by preventing them from receiving the ball or obstructing their plays when they do have the ball,"@en ;
                                             rdfs:label "markingAct"@en .


###  http://purl.obolibrary.org/obo/FutOn_00007
<http://purl.obolibrary.org/obo/FutOn_00007> rdf:type owl:Class ;
                                             rdfs:subClassOf <http://purl.obolibrary.org/obo/FutOn_00006> ;
                                             <http://purl.obolibrary.org/obo/IAO_0000115> "is a markingAct where a defender is responsible for guarding a specific area of the pitch, rather than a specific player. The defender attempts to intercept any opponent or ball that enters their zone."@en ;
                                             rdfs:label "manMarkingAct"@en .


###  http://purl.obolibrary.org/obo/FutOn_00008
<http://purl.obolibrary.org/obo/FutOn_00008> rdf:type owl:Class ;
                                             rdfs:subClassOf <http://purl.obolibrary.org/obo/FutOn_00006> ;
                                             <http://purl.obolibrary.org/obo/IAO_0000115> "a markingAct where a defender is assigned a specific player from the opposing team to guard, with the intent to limit their influence on the game. The defender typically shadows their assigned player, staying close and attempting to disrupt their play."@en ;
                                             rdfs:label "zonalMarkingAct"@en .


###  http://purl.obolibrary.org/obo/FutOn_00009
<http://purl.obolibrary.org/obo/FutOn_00009> rdf:type owl:Class ;
                                             rdfs:subClassOf <http://purl.obolibrary.org/obo/FutOn_00005> ;
                                             <http://purl.obolibrary.org/obo/IAO_0000115> "an outOfPossessionAct that is performed by a player when they attempt to dispossess an opponent by physically challenging them for the ball."@en ;
                                             rdfs:label "tackleAct"@en .


###  http://purl.obolibrary.org/obo/FutOn_00010
<http://purl.obolibrary.org/obo/FutOn_00010> rdf:type owl:Class ;
                                             rdfs:subClassOf <http://purl.obolibrary.org/obo/FutOn_00009> ;
                                             <http://purl.obolibrary.org/obo/IAO_0000115> "a tackleAct that is performed by a player when they position themselves in the path of the ball, typically while it is being shot or passed by an opponent, in an attempt to stop its progress or change its direction."@en ;
                                             rdfs:label "blockTackleAct"@en .


###  http://purl.obolibrary.org/obo/FutOn_00011
<http://purl.obolibrary.org/obo/FutOn_00011> rdf:type owl:Class ;
                                             rdfs:subClassOf <http://purl.obolibrary.org/obo/FutOn_00009> ;
                                             <http://purl.obolibrary.org/obo/IAO_0000115> "a tackleAct that is performed by a player when they slide on the ground to challenge an opponent for the ball, typically with one leg extended."@en ;
                                             rdfs:label "slideTackleAct"@en .


###  http://purl.obolibrary.org/obo/FutOn_00012
<http://purl.obolibrary.org/obo/FutOn_00012> rdf:type owl:Class ;
                                             rdfs:subClassOf <http://purl.obolibrary.org/obo/FutOn_00005> ;
                                             <http://purl.obolibrary.org/obo/IAO_0000115> "an outOfPossessionAct that is performed by a player when they disrupt an opponent's pass by moving into the ball's path, thereby gaining possession for their own team."@en ;
                                             rdfs:label "interceptionAct"@en .


###  http://purl.obolibrary.org/obo/FutOn_00013
<http://purl.obolibrary.org/obo/FutOn_00013> rdf:type owl:Class ;
                                             rdfs:subClassOf <http://purl.obolibrary.org/obo/FutOn_00004> ;
                                             <http://purl.obolibrary.org/obo/IAO_0000115> "inPossessionAct is a playerAct that involves actions executed by players of the team that currently has control of the ball."@en ;
                                             rdfs:label "inPossessionAct"@en .


###  http://purl.obolibrary.org/obo/FutOn_00014
<http://purl.obolibrary.org/obo/FutOn_00014> rdf:type owl:Class ;
                                             rdfs:subClassOf <http://purl.obolibrary.org/obo/FutOn_00006> ;
                                             <http://purl.obolibrary.org/obo/IAO_0000115> "rotationAct is an offBallAct that involves the strategic movement of a player who does not directly control the ball."@en ;
                                             rdfs:label "rotationAct"@en .


###  http://purl.obolibrary.org/obo/FutOn_00015
<http://purl.obolibrary.org/obo/FutOn_00015> rdf:type owl:Class ;
                                             rdfs:subClassOf <http://purl.obolibrary.org/obo/FutOn_00014> ;
                                             <http://purl.obolibrary.org/obo/IAO_0000115> "symmetricalRotationAct in football is a rotationAct that describes a strategic movement or action in which players rotate and change position in a manner that maintains symmetry about an axis."@en ;
                                             rdfs:label "symmetricalRotationAct"@en .


###  http://purl.obolibrary.org/obo/FutOn_00016
<http://purl.obolibrary.org/obo/FutOn_00016> rdf:type owl:Class ;
                                             rdfs:subClassOf <http://purl.obolibrary.org/obo/FutOn_00014> ;
                                             <http://purl.obolibrary.org/obo/IAO_0000115> "asymmetricalRotationAct in football is a rotationAct that describes a strategic movement or action in which players rotate and change position in a manner that does not maintain symmetry about an axis."@en ;
                                             rdfs:label "asymmetricalRotationAct"@en .


###  http://purl.obolibrary.org/obo/FutOn_00017
<http://purl.obolibrary.org/obo/FutOn_00017> rdf:type owl:Class ;
                                             rdfs:subClassOf <http://purl.obolibrary.org/obo/FutOn_00013> ;
                                             <http://purl.obolibrary.org/obo/IAO_0000115> "onBallAct is an inPossessionAct that involves a player maintaining control over the ball during gameplay."@en ;
                                             rdfs:label "onBallAct"@en .


###  http://purl.obolibrary.org/obo/FutOn_00018
<http://purl.obolibrary.org/obo/FutOn_00018> rdf:type owl:Class ;
                                             rdfs:subClassOf <http://purl.obolibrary.org/obo/FutOn_00017> ;
                                             <http://purl.obolibrary.org/obo/IAO_0000115> "shotAct is an onBallAct that is performed by a player when they attempt to propel the ball into the opponent's goal."@en ;
                                             rdfs:label "shotAct"@en .


###  http://purl.obolibrary.org/obo/FutOn_00019
<http://purl.obolibrary.org/obo/FutOn_00019> rdf:type owl:Class ;
                                             rdfs:subClassOf <http://purl.obolibrary.org/obo/FutOn_00018> ;
                                             <http://purl.obolibrary.org/obo/IAO_0000115> "bendingShotAct is a shotAct that is performed by a player when they strike the ball in a way that causes it to curve in the air."@en ;
                                             rdfs:label "bendingShotAct"@en .


###  http://purl.obolibrary.org/obo/FutOn_00020
<http://purl.obolibrary.org/obo/FutOn_00020> rdf:type owl:Class ;
                                             rdfs:subClassOf <http://purl.obolibrary.org/obo/FutOn_00018> ;
                                             <http://purl.obolibrary.org/obo/IAO_0000115> "bicycleShotAct is a shotAct that is performed by a player when they strike the ball in mid-air with a bicycle kick, a move where the player kicks the ball while performing a backflip."@en ;
                                             rdfs:label "bicycleShotAct"@en .


###  http://purl.obolibrary.org/obo/FutOn_00021
<http://purl.obolibrary.org/obo/FutOn_00021> rdf:type owl:Class ;
                                             rdfs:subClassOf <http://purl.obolibrary.org/obo/FutOn_00018> ;
                                             <http://purl.obolibrary.org/obo/IAO_0000115> "chipShotAct is a shotAct that is performed by a player when they strike the ball in an upward trajectory with the aim of lobbing it over the goalkeeper and into the net."@en ;
                                             rdfs:label "chipShotAct"@en .


###  http://purl.obolibrary.org/obo/FutOn_00022
<http://purl.obolibrary.org/obo/FutOn_00022> rdf:type owl:Class ;
                                             rdfs:subClassOf <http://purl.obolibrary.org/obo/FutOn_00018> ;
                                             <http://purl.obolibrary.org/obo/IAO_0000115> "headerShotAct is a shotAct that is performed by a player when they attempt to direct the ball into the opponent's goal by striking it with their head."@en ;
                                             rdfs:label "headerShotAct"@en .


###  http://purl.obolibrary.org/obo/FutOn_00023
<http://purl.obolibrary.org/obo/FutOn_00023> rdf:type owl:Class ;
                                             rdfs:subClassOf <http://purl.obolibrary.org/obo/FutOn_00018> ;
                                             <http://purl.obolibrary.org/obo/IAO_0000115> "rabonaShotAct is a shotAct that is performed by a player when they wrap their kicking leg around the back of their standing leg to strike the ball."@en ;
                                             rdfs:label "rabonaShotAct"@en .


###  http://purl.obolibrary.org/obo/FutOn_00024
<http://purl.obolibrary.org/obo/FutOn_00024> rdf:type owl:Class ;
                                             rdfs:subClassOf <http://purl.obolibrary.org/obo/FutOn_00018> ;
                                             <http://purl.obolibrary.org/obo/IAO_0000115> "standardShotAct is a shotAct that is performed by a player when they attempt to direct the ball into the opponent's goal by striking it with a standard kick, typically using the inside of the foot."@en ;
                                             rdfs:label "standardShotAct"@en .


###  http://purl.obolibrary.org/obo/FutOn_00025
<http://purl.obolibrary.org/obo/FutOn_00025> rdf:type owl:Class ;
                                             rdfs:subClassOf <http://purl.obolibrary.org/obo/FutOn_00018> ;
                                             <http://purl.obolibrary.org/obo/IAO_0000115> "straightShotAct is a shotAct that is performed by a player when they strike the ball in a straight trajectory towards the opponent's goal."@en ;
                                             rdfs:label "straightShotAct"@en .


###  http://purl.obolibrary.org/obo/FutOn_00026
<http://purl.obolibrary.org/obo/FutOn_00026> rdf:type owl:Class ;
                                             rdfs:subClassOf <http://purl.obolibrary.org/obo/FutOn_00018> ;
                                             <http://purl.obolibrary.org/obo/IAO_0000115> "volleyShotAct is a shotAct that is performed by a player when they strike the ball before it touches the ground, typically after a cross or a rebound."@en ;
                                             rdfs:label "volleyShotAct"@en .


###  http://purl.obolibrary.org/obo/FutOn_00031
<http://purl.obolibrary.org/obo/FutOn_00031> rdf:type owl:Class ;
                                             rdfs:subClassOf <http://purl.obolibrary.org/obo/FutOn_00015> ;
                                             <http://purl.obolibrary.org/obo/IAO_0000115> "dribbleAct is an onBallAct that involves a player controlling the ball and moving it forward by repeatedly striking it with any part legal part of their body."@en ;
                                             rdfs:label "dribbleAct"@en .


###  http://purl.obolibrary.org/obo/FutOn_00032
<http://purl.obolibrary.org/obo/FutOn_00032> rdf:type owl:Class ;
                                             rdfs:subClassOf <http://purl.obolibrary.org/obo/FutOn_00015> ;
                                             <http://purl.obolibrary.org/obo/IAO_0000115> "controlAct is an onBallAct that represents the action of a player successfully gaining possession of the ball from a pass or interception using any legal part of their body."@en ;
                                             rdfs:label "controlAct"@en .


###  http://purl.obolibrary.org/obo/FutOn_00033
<http://purl.obolibrary.org/obo/FutOn_00033> rdf:type owl:Class ;
                                             rdfs:subClassOf <http://purl.obolibrary.org/obo/FutOn_00032> ;
                                             <http://purl.obolibrary.org/obo/IAO_0000115> "chestControl is a controlAct that describes the action of a player successfully gaining possession of the ball using their chest."@en ;
                                             rdfs:label "chestControl"@en .


###  http://purl.obolibrary.org/obo/FutOn_00034
<http://purl.obolibrary.org/obo/FutOn_00034> rdf:type owl:Class ;
                                             rdfs:subClassOf <http://purl.obolibrary.org/obo/FutOn_00032> ;
                                             <http://purl.obolibrary.org/obo/IAO_0000115> "footControl is a controlAct that describes the action of a player successfully gaining possession of the ball using their foot."@en ;
                                             rdfs:label "footControl"@en .


###  http://purl.obolibrary.org/obo/FutOn_00035
<http://purl.obolibrary.org/obo/FutOn_00035> rdf:type owl:Class ;
                                             rdfs:subClassOf <http://purl.obolibrary.org/obo/FutOn_00015> ;
                                             <http://purl.obolibrary.org/obo/IAO_0000115> "passAct is an onBallAct in which a player, who is in control of the ball, deliberately sends the ball to a teammate."@en ;
                                             rdfs:label "passAct"@en .


###  http://purl.obolibrary.org/obo/FutOn_00036
<http://purl.obolibrary.org/obo/FutOn_00036> rdf:type owl:Class ;
                                             rdfs:subClassOf <http://purl.obolibrary.org/obo/FutOn_00035> ;
                                             <http://purl.obolibrary.org/obo/IAO_0000115> "crossAct is passAct that involves sending the ball across the field, usually from a wide position into the penalty area, aiming to reach a teammate."@en ;
                                             rdfs:label "crossAct"@en .


###  http://purl.obolibrary.org/obo/FutOn_00037
<http://purl.obolibrary.org/obo/FutOn_00037> rdf:type owl:Class ;
                                             rdfs:subClassOf <http://purl.obolibrary.org/obo/FutOn_00035> ;
                                             <http://purl.obolibrary.org/obo/IAO_0000115> "giveAndGoAct is a passAct that consists of a player passing the ball to a teammate and then immediately moving forward to receive a return pass."@en ;
                                             rdfs:label "giveAndGoAct"@en .


###  http://purl.obolibrary.org/obo/FutOn_00038
<http://purl.obolibrary.org/obo/FutOn_00038> rdf:type owl:Class ;
                                             rdfs:subClassOf <http://purl.obolibrary.org/obo/FutOn_00035> ;
                                             <http://purl.obolibrary.org/obo/IAO_0000115> "oneTouchPassAct is a passAct where the player passes the ball immediately upon receiving it, using just one touch."@en ;
                                             rdfs:label "oneTouchPassAct"@en .


###  http://purl.obolibrary.org/obo/FutOn_00039
<http://purl.obolibrary.org/obo/FutOn_00039> rdf:type owl:Class ;
                                             rdfs:subClassOf <http://purl.obolibrary.org/obo/FutOn_00035> ;
                                             <http://purl.obolibrary.org/obo/IAO_0000115> "throughPassAct is a passAct in which a player sends the ball through the opponents' defensive line to a teammate, typically to create a scoring opportunity."@en ;
                                             rdfs:label "throughPassAct"@en .


###  http://purl.obolibrary.org/obo/FutOn_00040
<http://purl.obolibrary.org/obo/FutOn_00040> rdf:type owl:Class ;
                                             rdfs:subClassOf <http://purl.obolibrary.org/obo/FutOn_00035> ;
                                             <http://purl.obolibrary.org/obo/IAO_0000115> "backHeelPassAct is a passAct that involves the player striking the ball with the back of their heel to pass it to a teammate, often employed to deceive the opposition."@en ;
                                             rdfs:label "backHeelPassAct"@en .


###  http://purl.obolibrary.org/obo/FutOn_00041
<http://purl.obolibrary.org/obo/FutOn_00041> rdf:type owl:Class ;
                                             rdfs:subClassOf <http://purl.obolibrary.org/obo/FutOn_00035> ;
                                             <http://purl.obolibrary.org/obo/IAO_0000115> "outsideFootPass is a passAct where the player uses the outside of their foot to pass the ball, typically to curve it around an opponent or for a change in direction."@en ;
                                             rdfs:label "outsideFootPass"@en .


###  http://purl.obolibrary.org/obo/FutOn_00042
<http://purl.obolibrary.org/obo/FutOn_00042> rdf:type owl:Class ;
                                             rdfs:subClassOf <http://purl.obolibrary.org/obo/FutOn_00035> ;
                                             <http://purl.obolibrary.org/obo/IAO_0000115> "pushPassAct is a passAct that involves the player using the inside of their foot to gently push the ball to a teammate, typically used for short, accurate passes."@en ;
                                             rdfs:label "pushPassAct"@en .


###  http://purl.obolibrary.org/obo/FutOn_00044
<http://purl.obolibrary.org/obo/FutOn_00044> rdf:type owl:Class ;
                                             rdfs:subClassOf <IAO:0000115/measurementInformationContentEntityFutOn10002> ;
                                             <http://purl.obolibrary.org/obo/IAO_0000115> "A measurementInformationContentEntity that quantifies or qualifies actions that take place in a game."@en ;
                                             rdfs:label "gameMeasurement"@en .


###  http://purl.obolibrary.org/obo/FutOn_00045
<http://purl.obolibrary.org/obo/FutOn_00045> rdf:type owl:Class ;
                                             rdfs:subClassOf <http://purl.obolibrary.org/obo/FutOn_00044> ;
                                             <http://purl.obolibrary.org/obo/IAO_0000115> "A gameMeasurement that represents a numeric or quantifiable property derived from a game or game-related event."@en ;
                                             rdfs:label "gameMeasurementQuantity"@en .


###  http://purl.obolibrary.org/obo/FutOn_00046
<http://purl.obolibrary.org/obo/FutOn_00046> rdf:type owl:Class ;
                                             rdfs:subClassOf <http://purl.obolibrary.org/obo/FutOn_00045> ;
                                             <http://purl.obolibrary.org/obo/IAO_0000115> "A gameMeasurementQuantity that quantifies the total number of successful tackles performed by a player or a team during a game."@en ;
                                             rdfs:label "tackleTally"@en .


###  http://purl.obolibrary.org/obo/FutOn_00047
<http://purl.obolibrary.org/obo/FutOn_00047> rdf:type owl:Class ;
                                             rdfs:subClassOf <http://purl.obolibrary.org/obo/FutOn_00045> ;
                                             <http://purl.obolibrary.org/obo/IAO_0000115> "A gameMeasurementQuantity that quantifies the total number of successful interceptions performed by a player or a team during a game."@en ;
                                             rdfs:label "interceptionTally"@en .


###  http://purl.obolibrary.org/obo/FutOn_00048
<http://purl.obolibrary.org/obo/FutOn_00048> rdf:type owl:Class ;
                                             rdfs:subClassOf <http://purl.obolibrary.org/obo/FutOn_00045> ;
                                             <http://purl.obolibrary.org/obo/IAO_0000115> "A gameMeasurementQuantity that quantifies the total number of successful goals scored by a player or a team during a game."@en ;
                                             rdfs:label "goalTally"@en .


###  http://purl.obolibrary.org/obo/FutOn_00049
<http://purl.obolibrary.org/obo/FutOn_00049> rdf:type owl:Class ;
                                             rdfs:subClassOf <http://purl.obolibrary.org/obo/FutOn_00045> ;
                                             <http://purl.obolibrary.org/obo/IAO_0000115> "A gameMeasurementQuantity that specifically quantifies the number of shots taken or made during a game."@en ;
                                             rdfs:label "shotTally"@en .


###  http://purl.obolibrary.org/obo/FutOn_00050
<http://purl.obolibrary.org/obo/FutOn_00050> rdf:type owl:Class ;
                                             rdfs:subClassOf <http://purl.obolibrary.org/obo/FutOn_00049> ;
                                             <http://purl.obolibrary.org/obo/IAO_0000115> "A shotTally that quantifies the total number of shots taken or made by an entire team during a game."@en ;
                                             rdfs:label "teamShotTally"@en .


###  http://purl.obolibrary.org/obo/FutOn_00051
<http://purl.obolibrary.org/obo/FutOn_00051> rdf:type owl:Class ;
                                             rdfs:subClassOf <http://purl.obolibrary.org/obo/FutOn_00049> ;
                                             <http://purl.obolibrary.org/obo/IAO_0000115> "A shotTally that quantifies the total number of shots taken or made by an individual player during a game."@en ;
                                             rdfs:label "playerShotTally"@en .


###  http://purl.obolibrary.org/obo/FutOn_00052
<http://purl.obolibrary.org/obo/FutOn_00052> rdf:type owl:Class ;
                                             rdfs:subClassOf <http://purl.obolibrary.org/obo/FutOn_00045> ;
                                             <http://purl.obolibrary.org/obo/IAO_0000115> "A gameMeasurementQuantity that specifically quantifies the total number of passes made during a game."@en ;
                                             rdfs:label "passTally"@en .


###  http://purl.obolibrary.org/obo/FutOn_00053
<http://purl.obolibrary.org/obo/FutOn_00053> rdf:type owl:Class ;
                                             rdfs:subClassOf <http://purl.obolibrary.org/obo/FutOn_00052> ;
                                             <http://purl.obolibrary.org/obo/IAO_0000115> "A passTally that quantifies the total number of passes made by an individual player during a game."@en ;
                                             rdfs:label "playerPassTally"@en .


###  http://purl.obolibrary.org/obo/FutOn_00054
<http://purl.obolibrary.org/obo/FutOn_00054> rdf:type owl:Class ;
                                             rdfs:subClassOf <http://purl.obolibrary.org/obo/FutOn_00052> ;
                                             <http://purl.obolibrary.org/obo/IAO_0000115> "A passTally that quantifies the total number of passes made by an entire team during a game or game-related event."@en ;
                                             rdfs:label "teamPassTally"@en .


###  http://purl.obolibrary.org/obo/FutOn_00055
<http://purl.obolibrary.org/obo/FutOn_00055> rdf:type owl:Class ;
                                             rdfs:subClassOf <http://purl.obolibrary.org/obo/FutOn_00045> ;
                                             <http://purl.obolibrary.org/obo/IAO_0000115> "A gameMeasurementQuantity that specifically represents the output of an xGAlgorithm, quantifying the probability of a shot resulting in a goal in a game."@en ;
                                             rdfs:label "xGValue"@en .


###  http://purl.obolibrary.org/obo/FutOn_00056
<http://purl.obolibrary.org/obo/FutOn_00056> rdf:type owl:Class ;
                                             rdfs:subClassOf <http://purl.obolibrary.org/obo/FutOn_00055> ;
                                             <http://purl.obolibrary.org/obo/IAO_0000115> "An xGValue that represents the xGValue for an individual player."@en ;
                                             rdfs:label "xGValuePlayer"@en .


###  http://purl.obolibrary.org/obo/FutOn_00057
<http://purl.obolibrary.org/obo/FutOn_00057> rdf:type owl:Class ;
                                             rdfs:subClassOf <http://purl.obolibrary.org/obo/FutOn_00055> ;
                                             <http://purl.obolibrary.org/obo/IAO_0000115> "An xGValue that represents the total Expected Goals (xG) value for a team in a game, calculated as the sum of the xGValues for all individual players on the team."@en ;
                                             rdfs:label "xGValueTeam"@en .


###  http://purl.obolibrary.org/obo/FutOn_00058
<http://purl.obolibrary.org/obo/FutOn_00058> rdf:type owl:Class ;
                                             rdfs:subClassOf <http://purl.obolibrary.org/obo/FutOn_00045> ;
                                             <http://purl.obolibrary.org/obo/IAO_0000115> "A gameMeasurementQuantity that quantifies the likelihood that a given pass will lead to a shot and subsequently a goal, based on various factors such as the type of pass, its origin and destination points, and the historical data."@en ;
                                             rdfs:label "xAValue"@en .


###  http://purl.obolibrary.org/obo/FutOn_00059
<http://purl.obolibrary.org/obo/FutOn_00059> rdf:type owl:Class ;
                                             rdfs:subClassOf <http://purl.obolibrary.org/obo/FutOn_00045> ;
                                             <http://purl.obolibrary.org/obo/IAO_0000115> "A gameMeasurementQuantity that quantifies the predicted number of points a team is expected to earn from a game based on the team's total xGValue, which is calculated from individual shot xGValues during the game."@en ;
                                             rdfs:label "xPValue"@en .


###  http://purl.obolibrary.org/obo/FutOn_00060
<http://purl.obolibrary.org/obo/FutOn_00060> rdf:type owl:Class ;
                                             rdfs:subClassOf <http://purl.obolibrary.org/obo/FutOn_00044> ;
                                             <http://purl.obolibrary.org/obo/IAO_0000115> "A gameMeasurement that specifically represents a qualitative or descriptive attribute associated with a game."@en ;
                                             rdfs:label "gameMeasurementQuality"@en .


###  http://purl.obolibrary.org/obo/FutOn_00061
<http://purl.obolibrary.org/obo/FutOn_00061> rdf:type owl:Class ;
                                             rdfs:subClassOf <http://purl.obolibrary.org/obo/FutOn_00060> ;
                                             <http://purl.obolibrary.org/obo/IAO_0000115> "A gameMeasurementQuality that involves a comprehensive evaluation of game dynamics, player performance, and team strategy, based on the xG values and potentially including other qualitative assessments."@en ;
                                             rdfs:label "xGAnalysis"@en .


###  http://purl.obolibrary.org/obo/FutOn_00062
<http://purl.obolibrary.org/obo/FutOn_00062> rdf:type owl:Class ;
                                             rdfs:subClassOf <http://purl.obolibrary.org/obo/FutOn_00060> ;
                                             <http://purl.obolibrary.org/obo/IAO_0000115> "A gameMeasurementQuality that assesses the quality of an individual player's performance during a game or game-related event, often on a scale (e.g., 1-10)."@en ;
                                             rdfs:label "playerPerformanceRating"@en .


###  http://purl.obolibrary.org/obo/FutOn_00063
<http://purl.obolibrary.org/obo/FutOn_00063> rdf:type owl:Class ;
                                             rdfs:subClassOf <http://purl.obolibrary.org/obo/FutOn_00060> ;
                                             <http://purl.obolibrary.org/obo/IAO_0000115> "A gameMeasurementQuality that identifies a specific phase or period of a game or game-related event (e.g., first half, second half, overtime)."@en ;
                                             rdfs:label "gamePhaseIdentification"@en .


###  http://purl.obolibrary.org/obo/FutOn_00064
<http://purl.obolibrary.org/obo/FutOn_00064> rdf:type owl:Class ;
                                             rdfs:subClassOf <http://purl.obolibrary.org/obo/FutOn_00060> ;
                                             <http://purl.obolibrary.org/obo/IAO_0000115> "A gameMeasurementQuality that represents an evaluation of the effectiveness of a player's markingAct in a game. This may be quantified by a number of factors, including but not limited to the number of times the marked opponent was dispossessed, the number of unsuccessful plays made by the marked opponent, the marked opponent's influence on the game relative to their average performance, and the outcome of the game."@en ;
                                             rdfs:label "markingQuality"@en .


###  http://purl.obolibrary.org/obo/FutOn_00065
<http://purl.obolibrary.org/obo/FutOn_00065> rdf:type owl:Class ;
                                             rdfs:subClassOf <IAO:0000115/AlgorithmFutOn:10000FutOn:10000> ;
                                             <http://purl.obolibrary.org/obo/IAO_0000115> "An Algorithm that is specifically designed to take as input data about a shot, such as its distance, angle, context (e.g., open play, set-piece, etc.), and potentially other factors, and output an xGValue."@en ;
                                             rdfs:label "xGAlgorithm"@en .


###  http://purl.obolibrary.org/obo/FutOn_00066
<http://purl.obolibrary.org/obo/FutOn_00066> rdf:type owl:Class ;
                                             rdfs:subClassOf <IAO:0000115/AlgorithmFutOn:10000FutOn:10000> ;
                                             <http://purl.obolibrary.org/obo/IAO_0000115> "An Algorithm that is specifically designed to take as input data about a pass, such as its type, origin and destination points, and other contextual factors, and output an xAValue, which quantifies the likelihood that the given pass will lead to a shot and subsequently a goal."@en ;
                                             rdfs:label "xAAlgorithm"@en .


###  http://purl.obolibrary.org/obo/FutOn_00068
<http://purl.obolibrary.org/obo/FutOn_00068> rdf:type owl:Class ;
                                             rdfs:subClassOf <IAO:0000115/PredictiveInformationContentEntityFutOn:10003> ;
                                             <http://purl.obolibrary.org/obo/IAO_0000115> "A PredictiveInformationContentEntity used to predict the outcome of a football match or series of matches, based on the sum of Expected Goals (xG) values of a team. It predicts the number of points a team is likely to earn from the match(es)."@en ;
                                             rdfs:label "xPForGamblers"@en .


###  http://purl.obolibrary.org/obo/FutOn_00069
<http://purl.obolibrary.org/obo/FutOn_00069> rdf:type owl:Class ;
                                             rdfs:subClassOf <IAO:0000115/PredictiveInformationContentEntityFutOn:10003> ;
                                             <http://purl.obolibrary.org/obo/IAO_0000115> "A PredictiveInformationContentEntity used to predict the outcome of a football match, based on the quantity and quality of shots taken by a team or player. It quantifies the probability of each shot resulting in a goal, considering various factors like distance from the goal, angle to the goal, game context, and historical data."@en ;
                                             rdfs:label "xGforGamblers"@en .


###  http://purl.obolibrary.org/obo/FutOn_00070
<http://purl.obolibrary.org/obo/FutOn_00070> rdf:type owl:Class ;
                                             rdfs:subClassOf <IAO:0000115/IdeologyFutOn:10001> ;
                                             <http://purl.obolibrary.org/obo/IAO_0000115> "An Ideology that represents the guiding principles, values, and strategic approach a football club adopts and adheres to in its operations, including player development, game strategy, and club management."@en ;
                                             rdfs:label "clubPhilosophy"@en .


###  http://purl.obolibrary.org/obo/FutOn_00071
<http://purl.obolibrary.org/obo/FutOn_00071> rdf:type owl:Class ;
                                             rdfs:subClassOf <http://purl.obolibrary.org/obo/FutOn_00070> ;
                                             <http://purl.obolibrary.org/obo/IAO_0000115> "A clubPhilosophy that emphasizes the use of Expected Goals (xG) metrics in various aspects of the football club's operations and strategy, including player performance analysis, team strategy, talent scouting, and player training."@en ;
                                             rdfs:label "xGPhilosophy"@en .


###  http://www.semanticweb.org/carte/ontologies/2023/6/untitled-ontology-63/FutOn:00001
<http://www.semanticweb.org/carte/ontologies/2023/6/untitled-ontology-63/FutOn:00001> rdf:type owl:Class ;
                                                                                      rdfs:subClassOf <IAO:0000115/IntentionalAct> ;
                                                                                      <http://purl.obolibrary.org/obo/IAO_0000115> "an intentionalAct that represents any action deliberately performed by an individual—such as a player, coach, or referee—during a game. These actions can range from playing actions (like shooting, passing, or tackling) performed by players, to strategic decisions and instructions given by coaches, to rulings and decisions made by referees."@en ;
                                                                                      rdfs:label "intentionalGameAct"@en .


###  Generated by the OWL API (version 4.5.9.2019-02-01T07:24:44Z) https://github.com/owlcs/owlapi
