@prefix : <http://www.semanticweb.org/carte/ontologies/2023/6/untitled-ontology-63#> .
@prefix obo: <http://purl.obolibrary.org/obo/> .
@prefix owl: <http://www.w3.org/2002/07/owl#> .
@prefix rdf: <http://www.w3.org/1999/02/22-rdf-syntax-ns#> .
@prefix xml: <http://www.w3.org/XML/1998/namespace> .
@prefix xsd: <http://www.w3.org/2001/XMLSchema#> .
@prefix rdfs: <http://www.w3.org/2000/01/rdf-schema#> .
@base <http://www.semanticweb.org/CarterBenson/FutOn/Prov/Definitions> .

<http://www.semanticweb.org/CarterBenson/FutOn/Prov/Definitions> rdf:type owl:Ontology .

#################################################################
#    Annotation properties
#################################################################

###  http://purl.obolibrary.org/obo/IAO_0000115
obo:IAO_0000115 rdf:type owl:AnnotationProperty ;
                rdfs:label "defintion"@en .


#################################################################
#    Classes
#################################################################

###  IAO:0000115/onPitchAct
<IAO:0000115/onPitchAct> rdf:type owl:Class ;
                         rdfs:subClassOf obo:FutOn_00004 .


###  http://purl.obolibrary.org/obo/FutOn_00002
obo:FutOn_00002 rdf:type owl:Class ;
                rdfs:subClassOf <http://www.semanticweb.org/carte/ontologies/2023/6/untitled-ontology-63/FutOn:00001> ;
                obo:IAO_0000115 "an intentionalMatchAct that represents any action deliberately performed by a referee during amatch."@en ;
                rdfs:comment "These actions can include making decisions on rule infractions, starting and stopping play, time-keeping, and any other actions aimed at enforcing the rules of thematch and ensuring fair play."@en ;
                rdfs:label "refereeAct"@en .


###  http://purl.obolibrary.org/obo/FutOn_00003
obo:FutOn_00003 rdf:type owl:Class ;
                rdfs:subClassOf <http://www.semanticweb.org/carte/ontologies/2023/6/untitled-ontology-63/FutOn:00001> ;
                obo:IAO_0000115 "an intentionalMatchAct that represents any action deliberately performed by a team's manager or coach during amatch."@en ;
                rdfs:comment "These actions can include strategic decisions, substitutions, tactical instructions, and any other actions aimed at guiding the team's play and strategy."@en ;
                rdfs:label "managerAct"@en .


###  http://purl.obolibrary.org/obo/FutOn_00004
obo:FutOn_00004 rdf:type owl:Class ;
                rdfs:subClassOf <http://www.semanticweb.org/carte/ontologies/2023/6/untitled-ontology-63/FutOn:00001> ;
                obo:IAO_0000115 "an intentionalMatchAct that represents any action performed intentionally by a player during amatch."@en ;
                rdfs:label "playerAct"@en .


###  http://purl.obolibrary.org/obo/FutOn_00005
obo:FutOn_00005 rdf:type owl:Class ;
                rdfs:subClassOf <IAO:0000115/onPitchAct> ;
                obo:IAO_0000115 "is a playerAct that involves actions taken by a player when their team does not have control of the ball."@en ;
                rdfs:label "outOfPossessionAct"@en .


###  http://purl.obolibrary.org/obo/FutOn_00006
obo:FutOn_00006 rdf:type owl:Class ;
                rdfs:subClassOf obo:FutOn_00005 ;
                obo:IAO_0000115 "an outOfPossessionAct, that involves a player positioning themselves close to a specific opposing player with the intent of limiting their influence on thematch by preventing them from receiving the ball or obstructing their plays when they do have the ball,"@en ;
                rdfs:label "markingAct"@en .


###  http://purl.obolibrary.org/obo/FutOn_00007
obo:FutOn_00007 rdf:type owl:Class ;
                rdfs:subClassOf obo:FutOn_00006 ;
                obo:IAO_0000115 "is a markingAct where a defender is responsible for guarding a specific area of the pitch, rather than a specific player. The defender attempts to intercept any opponent or ball that enters their zone."@en ;
                rdfs:label "manMarkingAct"@en .


###  http://purl.obolibrary.org/obo/FutOn_00008
obo:FutOn_00008 rdf:type owl:Class ;
                rdfs:subClassOf obo:FutOn_00006 ;
                obo:IAO_0000115 "a markingAct where a defender is assigned a specific player from the opposing team to guard, with the intent to limit their influence on thematch. The defender typically shadows their assigned player, staying close and attempting to disrupt their play."@en ;
                rdfs:label "zonalMarkingAct"@en .


###  http://purl.obolibrary.org/obo/FutOn_00009
obo:FutOn_00009 rdf:type owl:Class ;
                rdfs:subClassOf obo:FutOn_00005 ;
                obo:IAO_0000115 "an outOfPossessionAct that is performed by a player when they attempt to dispossess an opponent by physically challenging them for the ball."@en ;
                rdfs:label "tackleAct"@en .


###  http://purl.obolibrary.org/obo/FutOn_00010
obo:FutOn_00010 rdf:type owl:Class ;
                rdfs:subClassOf obo:FutOn_00009 ;
                obo:IAO_0000115 "a tackleAct that is performed by a player when they position themselves in the path of the ball, typically while it is being shot or passed by an opponent, in an attempt to stop its progress or change its direction."@en ;
                rdfs:label "blockTackleAct"@en .


###  http://purl.obolibrary.org/obo/FutOn_00011
obo:FutOn_00011 rdf:type owl:Class ;
                rdfs:subClassOf obo:FutOn_00009 ;
                obo:IAO_0000115 "a tackleAct that is performed by a player when they slide on the ground to challenge an opponent for the ball, typically with one leg extended."@en ;
                rdfs:label "slideTackleAct"@en .


###  http://purl.obolibrary.org/obo/FutOn_00012
obo:FutOn_00012 rdf:type owl:Class ;
                rdfs:subClassOf obo:FutOn_00005 ;
                obo:IAO_0000115 "an outOfPossessionAct that is performed by a player when they disrupt an opponent's pass by moving into the ball's path, thereby gaining possession for their own team."@en ;
                rdfs:label "interceptionAct"@en .


###  http://purl.obolibrary.org/obo/FutOn_00013
obo:FutOn_00013 rdf:type owl:Class ;
                rdfs:subClassOf <IAO:0000115/onPitchAct> ;
                obo:IAO_0000115 "inPossessionAct is a playerAct that involves actions executed by players of the team that currently has control of the ball."@en ;
                rdfs:label "inPossessionAct"@en .


###  http://purl.obolibrary.org/obo/FutOn_00014
obo:FutOn_00014 rdf:type owl:Class ;
                rdfs:subClassOf obo:FutOn_00112 ;
                obo:IAO_0000115 "rotationAct is an offBallAct that involves the strategic movement of a player who does not directly control the ball."@en ;
                rdfs:label "rotationAct"@en .


###  http://purl.obolibrary.org/obo/FutOn_00015
obo:FutOn_00015 rdf:type owl:Class ;
                rdfs:subClassOf obo:FutOn_00014 ;
                obo:IAO_0000115 "symmetricalRotationAct in football is a rotationAct that describes a strategic movement or action in which players rotate and change position in a manner that maintains symmetry about an axis."@en ;
                rdfs:label "symmetricalRotationAct"@en .


###  http://purl.obolibrary.org/obo/FutOn_00016
obo:FutOn_00016 rdf:type owl:Class ;
                rdfs:subClassOf obo:FutOn_00014 ;
                obo:IAO_0000115 "asymmetricalRotationAct in football is a rotationAct that describes a strategic movement or action in which players rotate and change position in a manner that does not maintain symmetry about an axis."@en ;
                rdfs:label "asymmetricalRotationAct"@en .


###  http://purl.obolibrary.org/obo/FutOn_00017
obo:FutOn_00017 rdf:type owl:Class ;
                rdfs:subClassOf obo:FutOn_00013 ;
                obo:IAO_0000115 "onBallAct is an inPossessionAct that involves a player maintaining control over the ball duringmatchplay."@en ;
                rdfs:label "onBallAct"@en .


###  http://purl.obolibrary.org/obo/FutOn_00018
obo:FutOn_00018 rdf:type owl:Class ;
                rdfs:subClassOf obo:FutOn_00017 ;
                obo:IAO_0000115 "shotAct is an onBallAct that is performed by a player when they attempt to propel the ball into the opponent's goal."@en ;
                rdfs:label "shotAct"@en .


###  http://purl.obolibrary.org/obo/FutOn_00019
obo:FutOn_00019 rdf:type owl:Class ;
                rdfs:subClassOf obo:FutOn_00018 ;
                obo:IAO_0000115 "bendingShotAct is a shotAct that is performed by a player when they strike the ball in a way that causes it to curve in the air."@en ;
                rdfs:label "bendingShotAct"@en .


###  http://purl.obolibrary.org/obo/FutOn_00020
obo:FutOn_00020 rdf:type owl:Class ;
                rdfs:subClassOf obo:FutOn_00018 ;
                obo:IAO_0000115 "bicycleShotAct is a shotAct that is performed by a player when they strike the ball in mid-air with a bicycle kick, a move where the player kicks the ball while performing a backflip."@en ;
                rdfs:label "bicycleShotAct"@en .


###  http://purl.obolibrary.org/obo/FutOn_00021
obo:FutOn_00021 rdf:type owl:Class ;
                rdfs:subClassOf obo:FutOn_00018 ;
                obo:IAO_0000115 "chipShotAct is a shotAct that is performed by a player when they strike the ball in an upward trajectory with the aim of lobbing it over the goalkeeper and into the net."@en ;
                rdfs:label "chipShotAct"@en .


###  http://purl.obolibrary.org/obo/FutOn_00022
obo:FutOn_00022 rdf:type owl:Class ;
                rdfs:subClassOf obo:FutOn_00018 ;
                obo:IAO_0000115 "headerShotAct is a shotAct that is performed by a player when they attempt to direct the ball into the opponent's goal by striking it with their head."@en ;
                rdfs:label "headerShotAct"@en .


###  http://purl.obolibrary.org/obo/FutOn_00023
obo:FutOn_00023 rdf:type owl:Class ;
                rdfs:subClassOf obo:FutOn_00018 ;
                obo:IAO_0000115 "rabonaShotAct is a shotAct that is performed by a player when they wrap their kicking leg around the back of their standing leg to strike the ball."@en ;
                rdfs:label "rabonaShotAct"@en .


###  http://purl.obolibrary.org/obo/FutOn_00024
obo:FutOn_00024 rdf:type owl:Class ;
                rdfs:subClassOf obo:FutOn_00018 ;
                obo:IAO_0000115 "standardShotAct is a shotAct that is performed by a player when they attempt to direct the ball into the opponent's goal by striking it with a standard kick, typically using the inside of the foot."@en ;
                rdfs:label "standardShotAct"@en .


###  http://purl.obolibrary.org/obo/FutOn_00025
obo:FutOn_00025 rdf:type owl:Class ;
                rdfs:subClassOf obo:FutOn_00018 ;
                obo:IAO_0000115 "straightShotAct is a shotAct that is performed by a player when they strike the ball in a straight trajectory towards the opponent's goal."@en ;
                rdfs:label "straightShotAct"@en .


###  http://purl.obolibrary.org/obo/FutOn_00026
obo:FutOn_00026 rdf:type owl:Class ;
                rdfs:subClassOf obo:FutOn_00018 ;
                obo:IAO_0000115 "volleyShotAct is a shotAct that is performed by a player when they strike the ball before it touches the ground, typically after a cross or a rebound."@en ;
                rdfs:label "volleyShotAct"@en .


###  http://purl.obolibrary.org/obo/FutOn_00031
obo:FutOn_00031 rdf:type owl:Class ;
                rdfs:subClassOf obo:FutOn_00015 ;
                obo:IAO_0000115 "dribbleAct is an onBallAct that involves a player controlling the ball and moving it forward by repeatedly striking it with any part legal part of their body."@en ;
                rdfs:label "dribbleAct"@en .


###  http://purl.obolibrary.org/obo/FutOn_00032
obo:FutOn_00032 rdf:type owl:Class ;
                rdfs:subClassOf obo:FutOn_00015 ;
                obo:IAO_0000115 "controlAct is an onBallAct that represents the action of a player successfully gaining possession of the ball from a pass or interception using any legal part of their body."@en ;
                rdfs:label "controlAct"@en .


###  http://purl.obolibrary.org/obo/FutOn_00033
obo:FutOn_00033 rdf:type owl:Class ;
                rdfs:subClassOf obo:FutOn_00032 ;
                obo:IAO_0000115 "chestControl is a controlAct that describes the action of a player successfully gaining possession of the ball using their chest."@en ;
                rdfs:label "chestControl"@en .


###  http://purl.obolibrary.org/obo/FutOn_00034
obo:FutOn_00034 rdf:type owl:Class ;
                rdfs:subClassOf obo:FutOn_00032 ;
                obo:IAO_0000115 "footControl is a controlAct that describes the action of a player successfully gaining possession of the ball using their foot."@en ;
                rdfs:label "footControl"@en .


###  http://purl.obolibrary.org/obo/FutOn_00035
obo:FutOn_00035 rdf:type owl:Class ;
                rdfs:subClassOf obo:FutOn_00015 ;
                obo:IAO_0000115 "passAct is an onBallAct in which a player, who is in control of the ball, deliberately sends the ball to a teammate."@en ;
                rdfs:label "passAct"@en .


###  http://purl.obolibrary.org/obo/FutOn_00036
obo:FutOn_00036 rdf:type owl:Class ;
                rdfs:subClassOf obo:FutOn_00035 ;
                obo:IAO_0000115 "crossAct is passAct that involves sending the ball across the field, usually from a wide position into the penalty area, aiming to reach a teammate."@en ;
                rdfs:label "crossAct"@en .


###  http://purl.obolibrary.org/obo/FutOn_00037
obo:FutOn_00037 rdf:type owl:Class ;
                rdfs:subClassOf obo:FutOn_00035 ;
                obo:IAO_0000115 "giveAndGoAct is a passAct that consists of a player passing the ball to a teammate and then immediately moving forward to receive a return pass."@en ;
                rdfs:label "giveAndGoAct"@en .


###  http://purl.obolibrary.org/obo/FutOn_00038
obo:FutOn_00038 rdf:type owl:Class ;
                rdfs:subClassOf obo:FutOn_00035 ;
                obo:IAO_0000115 "oneTouchPassAct is a passAct where the player passes the ball immediately upon receiving it, using just one touch."@en ;
                rdfs:label "oneTouchPassAct"@en .


###  http://purl.obolibrary.org/obo/FutOn_00039
obo:FutOn_00039 rdf:type owl:Class ;
                rdfs:subClassOf obo:FutOn_00035 ;
                obo:IAO_0000115 "throughPassAct is a passAct in which a player sends the ball through the opponents' defensive line to a teammate, typically to create a scoring opportunity."@en ;
                rdfs:label "throughPassAct"@en .


###  http://purl.obolibrary.org/obo/FutOn_00040
obo:FutOn_00040 rdf:type owl:Class ;
                rdfs:subClassOf obo:FutOn_00035 ;
                obo:IAO_0000115 "backHeelPassAct is a passAct that involves the player striking the ball with the back of their heel to pass it to a teammate, often employed to deceive the opposition."@en ;
                rdfs:label "backHeelPassAct"@en .


###  http://purl.obolibrary.org/obo/FutOn_00041
obo:FutOn_00041 rdf:type owl:Class ;
                rdfs:subClassOf obo:FutOn_00035 ;
                obo:IAO_0000115 "outsideFootPass is a passAct where the player uses the outside of their foot to pass the ball, typically to curve it around an opponent or for a change in direction."@en ;
                rdfs:label "outsideFootPass"@en .


###  http://purl.obolibrary.org/obo/FutOn_00042
obo:FutOn_00042 rdf:type owl:Class ;
                rdfs:subClassOf obo:FutOn_00035 ;
                obo:IAO_0000115 "pushPassAct is a passAct that involves the player using the inside of their foot to gently push the ball to a teammate, typically used for short, accurate passes."@en ;
                rdfs:label "pushPassAct"@en .


###  http://purl.obolibrary.org/obo/FutOn_00044
obo:FutOn_00044 rdf:type owl:Class ;
                rdfs:subClassOf <http://www.ontologyrepository.com/CommonCoreOntologies/MeasurementInformationContentEntity> ;
                obo:IAO_0000115 "A measurementInformationContentEntity that quantifies or qualifies actions that take place in amatch."@en ;
                rdfs:label "MatchMeasurement"@en .


###  http://purl.obolibrary.org/obo/FutOn_00045
obo:FutOn_00045 rdf:type owl:Class ;
                rdfs:subClassOf obo:FutOn_00044 ;
                obo:IAO_0000115 "AmatchMeasurement that represents a numeric or quantifiable property derived from amatch ormatch-related event."@en ;
                rdfs:label "MatchMeasurementQuantity"@en .


###  http://purl.obolibrary.org/obo/FutOn_00046
obo:FutOn_00046 rdf:type owl:Class ;
                rdfs:subClassOf obo:FutOn_00045 ;
                obo:IAO_0000115 "AmatchMeasurementQuantity that quantifies the total number of successful tackles performed by a player or a team during amatch."@en ;
                rdfs:label "tackleTally"@en .


###  http://purl.obolibrary.org/obo/FutOn_00047
obo:FutOn_00047 rdf:type owl:Class ;
                rdfs:subClassOf obo:FutOn_00045 ;
                obo:IAO_0000115 "AmatchMeasurementQuantity that quantifies the total number of successful interceptions performed by a player or a team during amatch."@en ;
                rdfs:label "interceptionTally"@en .


###  http://purl.obolibrary.org/obo/FutOn_00048
obo:FutOn_00048 rdf:type owl:Class ;
                rdfs:subClassOf obo:FutOn_00045 ;
                obo:IAO_0000115 "AmatchMeasurementQuantity that quantifies the total number of successful goals scored by a player or a team during amatch."@en ;
                rdfs:label "goalTally"@en .


###  http://purl.obolibrary.org/obo/FutOn_00049
obo:FutOn_00049 rdf:type owl:Class ;
                rdfs:subClassOf obo:FutOn_00045 ;
                obo:IAO_0000115 "AmatchMeasurementQuantity that specifically quantifies the number of shots taken or made during amatch."@en ;
                rdfs:label "shotTally"@en .


###  http://purl.obolibrary.org/obo/FutOn_00050
obo:FutOn_00050 rdf:type owl:Class ;
                rdfs:subClassOf obo:FutOn_00049 ;
                obo:IAO_0000115 "A shotTally that quantifies the total number of shots taken or made by an entire team during amatch."@en ;
                rdfs:label "teamShotTally"@en .


###  http://purl.obolibrary.org/obo/FutOn_00051
obo:FutOn_00051 rdf:type owl:Class ;
                rdfs:subClassOf obo:FutOn_00049 ;
                obo:IAO_0000115 "A shotTally that quantifies the total number of shots taken or made by an individual player during amatch."@en ;
                rdfs:label "playerShotTally"@en .


###  http://purl.obolibrary.org/obo/FutOn_00052
obo:FutOn_00052 rdf:type owl:Class ;
                rdfs:subClassOf obo:FutOn_00045 ;
                obo:IAO_0000115 "AmatchMeasurementQuantity that specifically quantifies the total number of passes made during amatch."@en ;
                rdfs:label "passTally"@en .


###  http://purl.obolibrary.org/obo/FutOn_00053
obo:FutOn_00053 rdf:type owl:Class ;
                rdfs:subClassOf obo:FutOn_00052 ;
                obo:IAO_0000115 "A passTally that quantifies the total number of passes made by an individual player during amatch."@en ;
                rdfs:label "playerPassTally"@en .


###  http://purl.obolibrary.org/obo/FutOn_00054
obo:FutOn_00054 rdf:type owl:Class ;
                rdfs:subClassOf obo:FutOn_00052 ;
                obo:IAO_0000115 "A passTally that quantifies the total number of passes made by an entire team during amatch ormatch-related event."@en ;
                rdfs:label "teamPassTally"@en .


###  http://purl.obolibrary.org/obo/FutOn_00055
obo:FutOn_00055 rdf:type owl:Class ;
                rdfs:subClassOf obo:FutOn_00045 ;
                obo:IAO_0000115 "AmatchMeasurementQuantity that specifically represents the output of an xGAlgorithm, quantifying the probability of a shot resulting in a goal in amatch."@en ;
                rdfs:label "xGValue"@en .


###  http://purl.obolibrary.org/obo/FutOn_00056
obo:FutOn_00056 rdf:type owl:Class ;
                rdfs:subClassOf obo:FutOn_00055 ;
                obo:IAO_0000115 "An xGValue that represents the xGValue for an individual player."@en ;
                rdfs:label "xGValuePlayer"@en .


###  http://purl.obolibrary.org/obo/FutOn_00057
obo:FutOn_00057 rdf:type owl:Class ;
                rdfs:subClassOf obo:FutOn_00055 ;
                obo:IAO_0000115 "An xGValue that represents the total Expected Goals (xG) value for a team in amatch, calculated as the sum of the xGValues for all individual players on the team."@en ;
                rdfs:label "xGValueTeam"@en .


###  http://purl.obolibrary.org/obo/FutOn_00058
obo:FutOn_00058 rdf:type owl:Class ;
                rdfs:subClassOf obo:FutOn_00045 ;
                obo:IAO_0000115 "AmatchMeasurementQuantity that quantifies the likelihood that a given pass will lead to a shot and subsequently a goal, based on various factors such as the type of pass, its origin and destination points, and the historical data."@en ;
                rdfs:label "xAValue"@en .


###  http://purl.obolibrary.org/obo/FutOn_00059
obo:FutOn_00059 rdf:type owl:Class ;
                rdfs:subClassOf obo:FutOn_00045 ;
                obo:IAO_0000115 "AmatchMeasurementQuantity that quantifies the predicted number of points a team is expected to earn from amatch based on the team's total xGValue, which is calculated from individual shot xGValues during thematch."@en ;
                rdfs:label "xPValue"@en .


###  http://purl.obolibrary.org/obo/FutOn_00060
obo:FutOn_00060 rdf:type owl:Class ;
                rdfs:subClassOf obo:FutOn_00044 ;
                obo:IAO_0000115 "AmatchMeasurement that specifically represents a qualitative or descriptive attribute associated with amatch."@en ;
                rdfs:label "MatchMeasurementQuality"@en .


###  http://purl.obolibrary.org/obo/FutOn_00061
obo:FutOn_00061 rdf:type owl:Class ;
                rdfs:subClassOf obo:FutOn_00060 ;
                obo:IAO_0000115 "AmatchMeasurementQuality that involves a comprehensive evaluation ofmatch dynamics, player performance, and team strategy, based on the xG values and potentially including other qualitative assessments."@en ;
                rdfs:label "xGAnalysis"@en .


###  http://purl.obolibrary.org/obo/FutOn_00062
obo:FutOn_00062 rdf:type owl:Class ;
                rdfs:subClassOf obo:FutOn_00060 ;
                obo:IAO_0000115 "AmatchMeasurementQuality that assesses the quality of an individual player's performance during amatch ormatch-related event, often on a scale (e.g., 1-10)."@en ;
                rdfs:label "playerPerformanceRating"@en .


###  http://purl.obolibrary.org/obo/FutOn_00063
obo:FutOn_00063 rdf:type owl:Class ;
                rdfs:subClassOf obo:FutOn_00060 ;
                obo:IAO_0000115 "AmatchMeasurementQuality that identifies a specific phase or period of amatch ormatch-related event (e.g., first half, second half, overtime)."@en ;
                rdfs:label "MatchPhaseIdentification"@en .


###  http://purl.obolibrary.org/obo/FutOn_00064
obo:FutOn_00064 rdf:type owl:Class ;
                rdfs:subClassOf obo:FutOn_00060 ;
                obo:IAO_0000115 "AmatchMeasurementQuality that represents an evaluation of the effectiveness of a player's markingAct in amatch. This may be quantified by a number of factors, including but not limited to the number of times the marked opponent was dispossessed, the number of unsuccessful plays made by the marked opponent, the marked opponent's influence on thematch relative to their average performance, and the outcome of thematch."@en ;
                rdfs:label "markingQuality"@en .


###  http://purl.obolibrary.org/obo/FutOn_00065
obo:FutOn_00065 rdf:type owl:Class ;
                rdfs:subClassOf <http://www.ontologyrepository.com/CommonCoreOntologies/Algorithm> ;
                obo:IAO_0000115 "An Algorithm that is specifically designed to take as input data about a shot, such as its distance, angle, context (e.g., open play, set-piece, etc.), and potentially other factors, and output an xGValue."@en ;
                rdfs:label "xGAlgorithm"@en .


###  http://purl.obolibrary.org/obo/FutOn_00066
obo:FutOn_00066 rdf:type owl:Class ;
                rdfs:subClassOf <http://www.ontologyrepository.com/CommonCoreOntologies/Algorithm> ;
                obo:IAO_0000115 "An Algorithm that is specifically designed to take as input data about a pass, such as its type, origin and destination points, and other contextual factors, and output an xAValue, which quantifies the likelihood that the given pass will lead to a shot and subsequently a goal."@en ;
                rdfs:label "xAAlgorithm"@en .


###  http://purl.obolibrary.org/obo/FutOn_00068
obo:FutOn_00068 rdf:type owl:Class ;
                rdfs:subClassOf <http://www.ontologyrepository.com/CommonCoreOntologies/PredictiveInformationContentEntity> ;
                obo:IAO_0000115 "A PredictiveInformationContentEntity used to predict the outcome of a footballmatch or series ofmatches, based on the sum of Expected Goals (xG) values of a team. It predicts the number of points a team is likely to earn from thematch(es)."@en ;
                rdfs:label "xPForGamblers"@en .


###  http://purl.obolibrary.org/obo/FutOn_00069
obo:FutOn_00069 rdf:type owl:Class ;
                rdfs:subClassOf <http://www.ontologyrepository.com/CommonCoreOntologies/PredictiveInformationContentEntity> ;
                obo:IAO_0000115 "A PredictiveInformationContentEntity used to predict the outcome of a footballmatch, based on the quantity and quality of shots taken by a team or player. It quantifies the probability of each shot resulting in a goal, considering various factors like distance from the goal, angle to the goal,match context, and historical data."@en ;
                rdfs:label "xGforGamblers"@en .


###  http://purl.obolibrary.org/obo/FutOn_00070
obo:FutOn_00070 rdf:type owl:Class ;
                rdfs:subClassOf <http://www.ontologyrepository.com/CommonCoreOntologies/Ideology> ;
                obo:IAO_0000115 "An Ideology that represents the guiding principles, values, and strategic approach a football club adopts and adheres to in its operations, including player development,match strategy, and club management."@en ;
                rdfs:label "clubPhilosophy"@en .


###  http://purl.obolibrary.org/obo/FutOn_00071
obo:FutOn_00071 rdf:type owl:Class ;
                rdfs:subClassOf obo:FutOn_00070 ;
                obo:IAO_0000115 "A clubPhilosophy that emphasizes the use of Expected Goals (xG) metrics in various aspects of the football club's operations and strategy, including player performance analysis, team strategy, talent scouting, and player training."@en ;
                rdfs:label "xGPhilosophy"@en .


###  http://purl.obolibrary.org/obo/FutOn_00074
obo:FutOn_00074 rdf:type owl:Class ;
                rdfs:subClassOf obo:FutOn_00002 ;
                obo:IAO_0000115 "A refereeAct that represents the action of making decisions on rule infractions during a game."@en ;
                rdfs:label "decisionAct"@en .


###  http://purl.obolibrary.org/obo/FutOn_00075
obo:FutOn_00075 rdf:type owl:Class ;
                rdfs:subClassOf obo:FutOn_00074 ;
                obo:IAO_0000115 "A decisionAct that represents the referee's action of making a decision related to fouls committed by players during a game."@en ;
                rdfs:label "foulDecisionAct"@en .


###  http://purl.obolibrary.org/obo/FutOn_00076
obo:FutOn_00076 rdf:type owl:Class ;
                rdfs:subClassOf obo:FutOn_00075 ;
                obo:IAO_0000115 "A foulDecisionAct that signifies the referee's action of making a decision regarding a suspected handball offense."@en ;
                rdfs:label "handballCall"@en .


###  http://purl.obolibrary.org/obo/FutOn_00077
obo:FutOn_00077 rdf:type owl:Class ;
                rdfs:subClassOf obo:FutOn_00075 ;
                obo:IAO_0000115 "A foulDecisionAct that signifies the referee's action of deciding on potential offside situations in a game."@en ;
                rdfs:label "offsideDecisionAct"@en .


###  http://purl.obolibrary.org/obo/FutOn_00078
obo:FutOn_00078 rdf:type owl:Class ;
                rdfs:subClassOf obo:FutOn_00075 ;
                obo:IAO_0000115 "A foulDecisionAct that encompasses the referee's action of deciding to issue a yellow or red card to a player."@en ;
                rdfs:label "cardDecisionAct"@en .


###  http://purl.obolibrary.org/obo/FutOn_00079
obo:FutOn_00079 rdf:type owl:Class ;
                rdfs:subClassOf obo:FutOn_00078 ;
                obo:IAO_0000115 "A cardDecisionAct that represents the referee's action of deciding to issue a yellow card to a player for a particular misconduct."@en ;
                rdfs:label "yellowCardDecisionAct"@en .


###  http://purl.obolibrary.org/obo/FutOn_00080
obo:FutOn_00080 rdf:type owl:Class ;
                rdfs:subClassOf obo:FutOn_00078 ;
                obo:IAO_0000115 "A cardDecisionAct that signifies the referee's action of deciding to issue a red card, either for a severe infraction or for a second yellow card offense in the same game."@en ;
                rdfs:label "redCardDecisionAct"@en .


###  http://purl.obolibrary.org/obo/FutOn_00081
obo:FutOn_00081 rdf:type owl:Class ;
                rdfs:subClassOf obo:FutOn_00002 ;
                obo:IAO_0000115 "A refereeAct that denotes the action of starting and stopping play during a game."@en ;
                rdfs:label "startingStoppingAct"@en .


###  http://purl.obolibrary.org/obo/FutOn_00082
obo:FutOn_00082 rdf:type owl:Class ;
                rdfs:subClassOf obo:FutOn_00081 ;
                obo:IAO_0000115 "A startingStoppingAct that signifies the referee's action of restarting the game after a foul has been addressed."@en ;
                rdfs:label "foulRestartAct"@en .


###  http://purl.obolibrary.org/obo/FutOn_00083
obo:FutOn_00083 rdf:type owl:Class ;
                rdfs:subClassOf obo:FutOn_00081 ;
                obo:IAO_0000115 "A startingStoppingAct that represents the referee's action of stopping the game due to a foul."@en ;
                rdfs:label "foulStopAct"@en .


###  http://purl.obolibrary.org/obo/FutOn_00084
obo:FutOn_00084 rdf:type owl:Class ;
                rdfs:subClassOf obo:FutOn_00081 ;
                obo:IAO_0000115 "A startingStoppingAct that represents the referee's action of initiating the start of a game."@en ;
                rdfs:label "gameStartAct"@en .


###  http://purl.obolibrary.org/obo/FutOn_00085
obo:FutOn_00085 rdf:type owl:Class ;
                rdfs:subClassOf obo:FutOn_00081 ;
                obo:IAO_0000115 "A startingStoppingAct that signifies the referee's action of calling the end of a game."@en ;
                rdfs:label "gameStopAct"@en .


###  http://purl.obolibrary.org/obo/FutOn_00086
obo:FutOn_00086 rdf:type owl:Class ;
                rdfs:subClassOf obo:FutOn_00081 ;
                obo:IAO_0000115 "A startingStoppingAct that denotes the referee's action of initiating the start of the second half of a game."@en ;
                rdfs:label "halfTimeStartAct"@en .


###  http://purl.obolibrary.org/obo/FutOn_00087
obo:FutOn_00087 rdf:type owl:Class ;
                rdfs:subClassOf obo:FutOn_00081 ;
                obo:IAO_0000115 "A startingStoppingAct that embodies the referee's action of declaring the end of the first half of a game."@en ;
                rdfs:label "halfTimeStopAct"@en .


###  http://purl.obolibrary.org/obo/FutOn_00088
obo:FutOn_00088 rdf:type owl:Class ;
                rdfs:subClassOf obo:FutOn_00002 ;
                obo:IAO_0000115 "A refereeAct that encompasses all actions related to keeping track of time during a game."@en ;
                rdfs:label "timeKeepingAct"@en .


###  http://purl.obolibrary.org/obo/FutOn_00089
obo:FutOn_00089 rdf:type owl:Class ;
                rdfs:subClassOf obo:FutOn_00088 ;
                obo:IAO_0000115 "A timeKeepingAct that represents the referee's action of monitoring the overall game clock."@en ;
                rdfs:label "gameClockMonitoringAct"@en .


###  http://purl.obolibrary.org/obo/FutOn_00090
obo:FutOn_00090 rdf:type owl:Class ;
                rdfs:subClassOf obo:FutOn_00088 ;
                obo:IAO_0000115 "A timeKeepingAct that denotes the referee's action of adding or subtracting stoppage time due to delays like injuries or interruptions."@en ;
                rdfs:label "stoppageTimeAdjustmentAct"@en .


###  http://purl.obolibrary.org/obo/FutOn_00091
obo:FutOn_00091 rdf:type owl:Class ;
                rdfs:subClassOf obo:FutOn_00088 ;
                obo:IAO_0000115 "A timeKeepingAct that signifies the referee's action of keeping track of the time elapsed in each half of the game."@en ;
                rdfs:label "halfTimeMonitoringAct"@en .


###  http://purl.obolibrary.org/obo/FutOn_00092
obo:FutOn_00092 rdf:type owl:Class ;
                rdfs:subClassOf obo:FutOn_00088 ;
                obo:IAO_0000115 "A timeKeepingAct that embodies the referee's action of keeping track of additional time periods in games that may go into extra time or overtime."@en ;
                rdfs:label "extraTimeMonitoringAct"@en .


###  http://purl.obolibrary.org/obo/FutOn_00093
obo:FutOn_00093 rdf:type owl:Class ;
                rdfs:subClassOf obo:FutOn_00002 ;
                obo:IAO_0000115 "A refereeAct that signifies actions aimed at enforcing the rules of the game and ensuring fair play."@en ;
                rdfs:label "fairPlayEnforcementAct"@en .


###  http://purl.obolibrary.org/obo/FutOn_00094
obo:FutOn_00094 rdf:type owl:Class ;
                rdfs:subClassOf obo:FutOn_00093 ;
                obo:IAO_0000115 "A fairPlayEnforcementAct that signifies the referee's action of penalizing player misconducts, in order to maintain fair play."@en ;
                rdfs:label "misconductPenalizingAct"@en .


###  http://purl.obolibrary.org/obo/FutOn_00095
obo:FutOn_00095 rdf:type owl:Class ;
                rdfs:subClassOf obo:FutOn_00093 ;
                obo:IAO_0000115 "A fairPlayEnforcementAct that denotes the referee's action of advocating for fair play, such as by managing player behavior, mediating disputes, or addressing unsportsmanlike conduct."@en ;
                rdfs:label "fairPlayAdvocacyAct"@en .


###  http://purl.obolibrary.org/obo/FutOn_00096
obo:FutOn_00096 rdf:type owl:Class ;
                rdfs:subClassOf obo:FutOn_00093 ;
                obo:IAO_0000115 "A fairPlayEnforcementAct that embodies the referee's action of controlling the overall game situation to ensure fair play, such as by managing player emotions, defusing tense situations, and so on."@en ;
                rdfs:label "gameControlAct"@en .


###  http://purl.obolibrary.org/obo/FutOn_00097
obo:FutOn_00097 rdf:type owl:Class ;
                rdfs:subClassOf obo:FutOn_00003 ;
                obo:IAO_0000115 "A managerAct that represents the action of selecting which players will start the game or be on the bench."@en ;
                rdfs:label "playerSelectionAct"@en .


###  http://purl.obolibrary.org/obo/FutOn_00098
obo:FutOn_00098 rdf:type owl:Class ;
                rdfs:subClassOf obo:FutOn_00003 ;
                obo:IAO_0000115 "A managerAct that signifies the manager's action of planning game strategies, deciding formations, and preparing tactical approaches."@en ;
                rdfs:label "strategyPlanningAct"@en .


###  http://purl.obolibrary.org/obo/FutOn_00099
obo:FutOn_00099 rdf:type owl:Class ;
                rdfs:subClassOf obo:FutOn_00003 ;
                obo:IAO_0000115 "A managerAct that denotes the manager's action of deciding when and which player should be substituted during a game."@en ;
                rdfs:label "substitutionAct"@en .


###  http://purl.obolibrary.org/obo/FutOn_00100
obo:FutOn_00100 rdf:type owl:Class ;
                rdfs:subClassOf obo:FutOn_00099 ;
                obo:IAO_0000115 "A substitutionAct that represents the manager's action of substituting a player due to injury."@en ;
                rdfs:label "injurySubstitutionAct"@en .


###  http://purl.obolibrary.org/obo/FutOn_00101
obo:FutOn_00101 rdf:type owl:Class ;
                rdfs:subClassOf obo:FutOn_00099 ;
                obo:IAO_0000115 "A substitutionAct that signifies the manager's action of substituting a player to implement a new tactical approach or to strengthen a particular area of the team."@en ;
                rdfs:label "tacticalSubstitutionAct"@en .


###  http://purl.obolibrary.org/obo/FutOn_00102
obo:FutOn_00102 rdf:type owl:Class ;
                rdfs:subClassOf obo:FutOn_00099 ;
                obo:IAO_0000115 "A substitutionAct that denotes the manager's action of substituting a player due to disciplinary issues, such as to prevent a player at risk of receiving a red card from being sent off."@en ;
                rdfs:label "disciplinarySubstitutionAct"@en .


###  http://purl.obolibrary.org/obo/FutOn_00103
obo:FutOn_00103 rdf:type owl:Class ;
                rdfs:subClassOf obo:FutOn_00099 ;
                obo:IAO_0000115 "A substitutionAct that represents the manager's action of substituting a player who is tired or not performing optimally due to fatigue."@en ;
                rdfs:label "fatigueSubstitutionAct"@en .


###  http://purl.obolibrary.org/obo/FutOn_00104
obo:FutOn_00104 rdf:type owl:Class ;
                rdfs:subClassOf obo:FutOn_00099 ;
                obo:IAO_0000115 "A substitutionAct that embodies the manager's action of substituting a player in order to waste time, usually towards the end of the game when the team is leading."@en ;
                rdfs:label "timeWastingSubstitutionAct"@en .


###  http://purl.obolibrary.org/obo/FutOn_00105
obo:FutOn_00105 rdf:type owl:Class ;
                rdfs:subClassOf obo:FutOn_00003 ;
                obo:IAO_0000115 "A managerAct that embodies the manager's action of communicating instructions, feedback, or motivational speeches to players."@en ;
                rdfs:label "communicationAct"@en .


###  http://purl.obolibrary.org/obo/FutOn_00106
obo:FutOn_00106 rdf:type owl:Class ;
                rdfs:subClassOf obo:FutOn_00003 ;
                obo:IAO_0000115 "A managerAct that represents the action of a manager analyzing the strategies, strengths, and weaknesses of opponent teams."@en ;
                rdfs:label "opponentAnalysisAct"@en .


###  http://purl.obolibrary.org/obo/FutOn_00107
obo:FutOn_00107 rdf:type owl:Class ;
                rdfs:subClassOf obo:FutOn_00098 ;
                obo:IAO_0000115 "A strategyPlanningAct that represents the manager's action of selecting the team's formation for a game."@en ;
                rdfs:label "formationSelectionAct"@en .


###  http://purl.obolibrary.org/obo/FutOn_00108
obo:FutOn_00108 rdf:type owl:Class ;
                rdfs:subClassOf obo:FutOn_00098 ;
                obo:IAO_0000115 "A strategyPlanningAct that signifies the manager's action of preparing set piece strategies, such as free kicks, corners, or penalty kicks."@en ;
                rdfs:label "setPiecePreparationAct"@en .


###  http://purl.obolibrary.org/obo/FutOn_00109
obo:FutOn_00109 rdf:type owl:Class ;
                rdfs:subClassOf obo:FutOn_00106 ;
                obo:IAO_0000115 "An opponentAnalysisAct that represents the manager's action of analyzing the strategies, strengths, and weaknesses of specific opponent teams."@en ;
                rdfs:label "oppositionAnalysisAct"@en .


###  http://purl.obolibrary.org/obo/FutOn_00110
obo:FutOn_00110 rdf:type owl:Class ;
                rdfs:subClassOf obo:FutOn_00106 ;
                obo:IAO_0000115 "An opponentAnalysisAct that signifies the manager's action of assessing individual players of the opponent team, their strengths, weaknesses, and playing styles."@en ;
                rdfs:label "playerAssessmentAct"@en .


###  http://purl.obolibrary.org/obo/FutOn_00111
obo:FutOn_00111 rdf:type owl:Class ;
                rdfs:subClassOf obo:FutOn_00097 ;
                obo:IAO_0000115 "A playerSelectionAct that represents the manager's action of selecting the squad for a game, including both the starting lineup and substitutes."@en ;
                rdfs:label "squadSelectionAct"@en .


###  http://purl.obolibrary.org/obo/FutOn_00112
obo:FutOn_00112 rdf:type owl:Class ;
                rdfs:subClassOf obo:FutOn_00013 ;
                obo:IAO_0000115 "An offBallAct that represents actions performed by a player when not in possession of the ball during a game."@en ;
                rdfs:label "offBallAct"@en .
##  http://purl.obolibrary.org/obo/FutOn_00113
:00113 rdf:type owl:Class ;
       rdfs:subClassOf :00014 ;
       obo:IAO_0000115 "A playerAct that represents any action intentionally performed by a substitute player or non-playing athlete from the bench during a match."@en ;
       rdfs:label "benchPlayerAct"@en .

##  http://purl.obolibrary.org/obo/FutOn_00114
:00114 rdf:type owl:Class ;
       rdfs:subClassOf :00113 ;
       obo:IAO_0000115 "A BenchPlayerAct that involves a substitute player or non-playing athlete vocally encouraging their team from the sidelines. This can include cheering, chanting, or offering positive affirmations."@en ;
       rdfs:label "benchPlayerCheeringAct"@en .

##  http://purl.obolibrary.org/obo/FutOn_00115
:00115 rdf:type owl:Class ;
       rdfs:subClassOf :00113 ;
       obo:IAO_0000115 "A BenchPlayerAct that involves a substitute player or non-playing athlete engaging in conversations about game tactics and strategies with other bench members or coaches."@en ;
       rdfs:label "benchPlayerStrategicDiscussionAct"@en .

##  http://purl.obolibrary.org/obo/FutOn_00116
:00116 rdf:type owl:Class ;
       rdfs:subClassOf :00113 ;
       obo:IAO_0000115 "A BenchPlayerAct that involves a substitute player or non-playing athlete performing physical activity to prepare for potential entry into the match. This can include activities like stretching, jogging, and sport-specific drills."@en ;
       rdfs:label "benchPlayerWarmUpAct"@en .

##  http://purl.obolibrary.org/obo/FutOn_00117
:00117 rdf:type owl:Class ;
       rdfs:subClassOf :00113 ;
       obo:IAO_0000115 "A BenchPlayerAct that involves a substitute player or non-playing athlete assisting the coaching staff in various ways, such as relaying messages to on-field players or contributing to tactical decisions."@en ;
       rdfs:label "benchPlayerCoachingAssistanceAct"@en .

##  http://purl.obolibrary.org/obo/FutOn_00118
:00118 rdf:type owl:Class ;
       rdfs:subClassOf :00113 ;
       obo:IAO_0000115 "A BenchPlayerAct that involves a substitute player or non-playing athlete preparing to enter the match as a substitute, often in response to a coach's decision or a teammate's injury."@en ;
       rdfs:label "benchPlayerSubstitutionReadinessAct"@en .

##  http://purl.obolibrary.org/obo/FutOn_00119
:00119 rdf:type owl:Class ;
       rdfs:subClassOf :00113 ;
       obo:IAO_0000115 "A BenchPlayerAct that involves a substitute player or non-playing athlete consuming fluids to maintain hydration levels during the match."@en ;
       rdfs:label "benchPlayerRehydrationAct"@en .

##  http://purl.obolibrary.org/obo/FutOn_00120
:00120 rdf:type owl:Class ;
       rdfs:subClassOf :00113 ;
       obo:IAO_0000115 "A BenchPlayerAct that involves a substitute player or non-playing athlete consuming energy-dense foods or supplements to maintain energy levels and readiness for potential match entry."@en ;
       rdfs:label "benchPlayerNutritionAct"@en .

##  http://purl.obolibrary.org/obo/FutOn_00121
:00121 rdf:type owl:Class ;
       rdfs:subClassOf :00014 ;
      obo:IAO_0000115 "An intentionalMatchAct that represents any action deliberately performed by an individual spectator during a match."@en ;
       rdfs:label "fanAct"@en .

##  http://purl.obolibrary.org/obo/FutOn_00122
:00122 rdf:type owl:Class ;
       rdfs:subClassOf :00121 ;
      obo:IAO_0000115 "A fanAct that involves vocal support, often in the form of shouting, chanting, or singing, aimed at encouraging a team or player."@en ;
       rdfs:label "cheeringAct"@en .

##  http://purl.obolibrary.org/obo/FutOn_00123
:00123 rdf:type owl:Class ;
       rdfs:subClassOf :00121 ;
      obo:IAO_0000115 "A fanAct that involves clapping hands to express approval, praise, or enthusiasm for a specific play or player."@en ;
       rdfs:label "applaudingAct"@en .

##  http://purl.obolibrary.org/obo/FutOn_00124
:00124 rdf:type owl:Class ;
       rdfs:subClassOf :00121 ;
      obo:IAO_0000115 "A fanAct that involves creating and showing banners or signs, usually to express support for a team or player, or to communicate a particular sentiment or message."@en ;
       rdfs:label "bannerDisplayingAct"@en .

##  http://purl.obolibrary.org/obo/FutOn_00125
:00125 rdf:type owl:Class ;
       rdfs:subClassOf :00121 ;
      obo:IAO_0000115 "A fanAct that involves posting on social media platforms about the match, typically to share views, express support, or engage with other fans."@en ;
       rdfs:label "socialMediaPostingAct"@en .

##  http://purl.obolibrary.org/obo/FutOn_00126
:00126 rdf:type owl:Class ;
       rdfs:subClassOf :00121 ;
      obo:IAO_0000115 "A fanAct that involves expressing disapproval or discontent, typically towards a particular player, team, or referee decision, by booing or jeering."@en ;
       rdfs:label "booingAct"@en .

##  http://purl.obolibrary.org/obo/FutOn_00127
:00127 rdf:type owl:Class ;
       rdfs:subClassOf :00121 ;
      obo:IAO_0000115 "A fanAct that involves intentional silence or non-participation in certain activities (like chants or applause) to express dissatisfaction or protest against an issue related to the match or the teams."@en ;
       rdfs:label "silentProtestAct"@en .

##  http://purl.obolibrary.org/obo/FutOn_00128
:00128 rdf:type owl:Class ;
       rdfs:subClassOf :00121 ;
      obo:IAO_0000115 "A fanAct that involves a spectator unlawfully entering the playing area during a match. This is generally considered dangerous and disrespectful, and it's usually strictly prohibited."@en ;
       rdfs:label "pitchInvasionAct"@en .

##  http://purl.obolibrary.org/obo/FutOn_00129
:00129 rdf:type owl:Class ;
       rdfs:subClassOf :00121 ;
      obo:IAO_0000115 "A fanAct that involves violent, disorderly, or destructive behavior, often resulting in harm to others or damage to property."@en ;
       rdfs:label "hooliganismAct"@en .

##  http://purl.obolibrary.org/obo/FutOn_00130
:00130 rdf:type owl:Class ;
       rdfs:subClassOf :00121 ;
      obo:IAO_0000115 "A fanAct that involves offensive, discriminatory, or hate-fueled chants or shouts. This can include racism, sexism, homophobia, and other forms of abuse."@en ;
       rdfs:label "abusiveChantingAct"@en .

##  http://purl.obolibrary.org/obo/FutOn_00131
:00131 rdf:type owl:Class ;
       rdfs:subClassOf :00121 ;
      obo:IAO_0000115 "A fanAct that involves throwing objects onto the pitch or at other spectators. This can be very dangerous and is usually strictly prohibited."@en ;
       rdfs:label "projectileThrowingAct"@en .

##  http://purl.obolibrary.org/obo/FutOn_00132
:00132 rdf:type owl:Class ;
       rdfs:subClassOf :00121 ;
      obo:IAO_0000115 "A fanAct that involves the intentional discomfort or harm of others through unwanted actions or behaviors, such as stalking or physical and verbal abuse."@en ;
       rdfs:label "harassmentAct"@en .

##  http://purl.obolibrary.org/obo/FutOn_00133
:00133 rdf:type owl:Class ;
       rdfs:subClassOf :00121 ;
      obo:IAO_0000115 "A fanAct that involves the deliberate damage or defacement of property, whether the venue's facilities, vehicles in the vicinity, or other fans' belongings."@en ;
       rdfs:label "vandalismAct"@en .

##  http://purl.obolibrary.org/obo/FutOn_00134
obo:FutOn_00134 rdf:type owl:Class ;
                rdfs:subClassOf obo:FutOn_00121 ;
                obo:IAO_0000115 "A playerPosition in which a player is responsible for guarding the team's goal and preventing the opposing team from scoring. This is the only position allowed to handle the ball within the penalty area."@en ;
                rdfs:label "goalkeeper"@en .

##  http://purl.obolibrary.org/obo/FutOn_00135
obo:FutOn_00135 rdf:type owl:Class ;
                rdfs:subClassOf obo:FutOn_00121 ;
                obo:IAO_0000115 "A playerPosition that involves a player primarily focusing on preventing the opposing team from scoring. Subclasses could include center-back, full-back, wing-back, and sweeper."@en ;
                rdfs:label "defender"@en .

##  http://purl.obolibrary.org/obo/FutOn_00136
obo:FutOn_00136 rdf:type owl:Class ;
                rdfs:subClassOf obo:FutOn_00135 ;
                obo:IAO_0000115 "A defender where the player occupies a central position in defense, typically focusing on intercepting passes, blocking shots, and marking opposing forwards."@en ;
                rdfs:label "centerBack"@en .

##  http://purl.obolibrary.org/obo/FutOn_00137
obo:FutOn_00137 rdf:type owl:Class ;
                rdfs:subClassOf obo:FutOn_00135 ;
                obo:IAO_0000115 "A defender where the player occupies the flanks of the defense, often contributing to both defensive tasks and attacking plays along the wings."@en ;
                rdfs:label "fullBack"@en .

##  http://purl.obolibrary.org/obo/FutOn_00138
obo:FutOn_00138 rdf:type owl:Class ;
                rdfs:subClassOf obo:FutOn_00137 ;
                obo:IAO_0000115 "A fullBack often used in formations that utilize three center-backs. These players patrol wide areas of the pitch, supporting both defensive and offensive tasks."@en ;
                rdfs:label "wingBack"@en .

##  http://purl.obolibrary.org/obo/FutOn_00139
obo:FutOn_00139 rdf:type owl:Class ;
                rdfs:subClassOf obo:FutOn_00135 ;
                obo:IAO_0000115 "A defender often positioned behind the line of defenders, focusing on clearing the ball from the defensive zone and covering defensive gaps."@en ;
                rdfs:label "sweeper"@en .

##  http://purl.obolibrary.org/obo/FutOn_00140
obo:FutOn_00140 rdf:type owl:Class ;
                rdfs:subClassOf obo:FutOn_00121 ;
                obo:IAO_0000115 "A player that involves a player operating in the area of the field between the defense and the forwards, often involved in both attacking and defensive duties. Subclasses could include central midfielder, attacking midfielder, defensive midfielder, and wide midfielder."@en ;
                rdfs:label "midfielder"@en .

##  http://purl.obolibrary.org/obo/FutOn_00141
obo:FutOn_00141 rdf:type owl:Class ;
                rdfs:subClassOf obo:FutOn_00140 ;
                obo:IAO_0000115 "A midfielder where the player is often involved in both attacking and defensive duties, distributing the ball, and maintaining possession."@en ;
                rdfs:label "centralMidfielder"@en .

##  http://purl.obolibrary.org/obo/FutOn_00142
obo:FutOn_00142 rdf:type owl:Class ;
                rdfs:subClassOf obo:FutOn_00140 ;
                obo:IAO_0000115 "A midfielder where the player is positioned closer to the forwards and focuses on creating scoring opportunities."@en ;
                rdfs:label "attackingMidfielder"@en .

##  http://purl.obolibrary.org/obo/FutOn_00143
obo:FutOn_00143 rdf:type owl:Class ;
                rdfs:subClassOf obo:FutOn_00140 ;
                obo:IAO_0000115 "A midfielder where the player is positioned closer to the defense and focuses on shielding the defensive line and disrupting opposing attacks."@en ;
                rdfs:label "defensiveMidfielder"@en .

##  http://purl.obolibrary.org/obo/FutOn_00144
obo:FutOn_00144 rdf:type owl:Class ;
                rdfs:subClassOf obo:FutOn_00140 ;
                obo:IAO_0000115 "A midfielder where the player occupies the flanks of the field, often contributing to both defensive tasks and attacking plays along the wings."@en ;
                rdfs:label "wideMidfielder"@en .

##  http://purl.obolibrary.org/obo/FutOn_00145
obo:FutOn_00145 rdf:type owl:Class ;
                rdfs:subClassOf obo:FutOn_00144 ;
                obo:IAO_0000115 "A wideMidfielder in which a player operates primarily on the left side of the field."@en ;
                rdfs:label "leftMidfielder"@en .

##  http://purl.obolibrary.org/obo/FutOn_00146
obo:FutOn_00146 rdf:type owl:Class ;
                rdfs:subClassOf obo:FutOn_00134 ;
                obo:IAO_0000115 "A playerPosition that involves a player primarily focusing on scoring goals and creating attacking opportunities."@en ;
                rdfs:label "forward"@en .

##  http://purl.obolibrary.org/obo/FutOn_00147
obo:FutOn_00147 rdf:type owl:Class ;
                rdfs:subClassOf obo:FutOn_00146 ;
                obo:IAO_0000115 "A forward where the player leads the attack by positioning centrally, often the primary target for scoring opportunities."@en ;
                rdfs:label "centerForward"@en .

##  http://purl.obolibrary.org/obo/FutOn_00148
obo:FutOn_00148 rdf:type owl:Class ;
                rdfs:subClassOf obo:FutOn_00146 ;
                obo:IAO_0000115 "A forward where the player supports the main striker, often dropping deeper into the midfield to receive the ball, turn, and run at the defense."@en ;
                rdfs:label "secondStriker"@en .

##  http://purl.obolibrary.org/obo/FutOn_00149
obo:FutOn_00149 rdf:type owl:Class ;
                rdfs:subClassOf obo:FutOn_00146 ;
                obo:IAO_0000115 "A forward where the player is positioned on the wide parts of the pitch, often focusing on delivering crosses into the penalty area."@en ;
                rdfs:label "winger"@en .

##  http://purl.obolibrary.org/obo/FutOn_00150
obo:FutOn_00150 rdf:type owl:Class ;
                rdfs:subClassOf obo:FutOn_00146 ;
                obo:IAO_0000115 "A forward where the player, while nominally a striker, drops deep into midfield to disrupt defensive lines and create space for teammates."@en ;
                rdfs:label "falseNine"@en .

###  http://www.ontologyrepository.com/CommonCoreOntologies/ActionPermission
<http://www.ontologyrepository.com/CommonCoreOntologies/ActionPermission> rdf:type owl:Class ;
                                                                          rdfs:subClassOf <http://www.ontologyrepository.com/CommonCoreOntologies/ActionRegulation> ;
                                                                          obo:IAO_0000115 "An Action Regulation that permits some Act."@en ;
                                                                          rdfs:label "Action Permission"@en .


###  http://www.ontologyrepository.com/CommonCoreOntologies/ActionProhibition
<http://www.ontologyrepository.com/CommonCoreOntologies/ActionProhibition> rdf:type owl:Class ;
                                                                           rdfs:subClassOf <http://www.ontologyrepository.com/CommonCoreOntologies/ActionRegulation> ;
                                                                           obo:IAO_0000115 "An Action Regulation that prohibits some Act."@en ;
                                                                           rdfs:label "Action Prohibition"@en .


###  http://www.ontologyrepository.com/CommonCoreOntologies/ActionRegulation
<http://www.ontologyrepository.com/CommonCoreOntologies/ActionRegulation> rdf:type owl:Class ;
                                                                          rdfs:subClassOf <http://www.ontologyrepository.com/CommonCoreOntologies/DirectiveInformationContentEntity> ;
                                                                          obo:IAO_0000115 "A Directive Information Content Entity that prescribes an Act as required, prohibited, or permitted, and is the output of an Act which realizes some Authority Role."@en ,
                                                                                          "Action Regulation"@en .


###  http://www.ontologyrepository.com/CommonCoreOntologies/ActionRequirement
<http://www.ontologyrepository.com/CommonCoreOntologies/ActionRequirement> rdf:type owl:Class ;
                                                                           rdfs:subClassOf <http://www.ontologyrepository.com/CommonCoreOntologies/ActionRegulation> ;
                                                                           obo:IAO_0000115 "An Action Regulation that requires some Act."@en ;
                                                                           rdfs:label "Action Requirement"@en .


###  http://www.ontologyrepository.com/CommonCoreOntologies/Algorithm
<http://www.ontologyrepository.com/CommonCoreOntologies/Algorithm> rdf:type owl:Class ;
                                                                   rdfs:subClassOf <http://www.ontologyrepository.com/CommonCoreOntologies/DirectiveInformationContentEntity> ;
                                                                   obo:IAO_0000115 "A Directive Information Content Entity that prescribes the inputs and output of mathematical functions as well as workflow of execution for achieving a predefined objective"@en ;
                                                                   rdfs:label "Algorithm" .


###  http://www.ontologyrepository.com/CommonCoreOntologies/DescriptiveInformationContentEntity
<http://www.ontologyrepository.com/CommonCoreOntologies/DescriptiveInformationContentEntity> rdf:type owl:Class ;
                                                                                             obo:IAO_0000115 "An Information Content Entity that consists of a set of propositions that describe some Entity."@en ;
                                                                                             rdfs:label "Descriptive Information Content Entity"@en .


###  http://www.ontologyrepository.com/CommonCoreOntologies/DirectiveInformationContentEntity
<http://www.ontologyrepository.com/CommonCoreOntologies/DirectiveInformationContentEntity> rdf:type owl:Class ;
                                                                                           obo:IAO_0000115 "An Information Content Entity that consists of a set of propositions or images (as in the case of a blueprint) that prescribe some Entity."@en ;
                                                                                           rdfs:label "Directive Information Content Entity"@en .


###  http://www.ontologyrepository.com/CommonCoreOntologies/Ideology
<http://www.ontologyrepository.com/CommonCoreOntologies/Ideology> rdf:type owl:Class ;
                                                                  obo:IAO_0000115 "An Information Content Entity that consists of a collection of claims about how some part of the world is or should be and which is accepted as true by an Agent or Group of Agents such that it forms the basis of their beliefs, goals, expectations, and motivations."@en ;
                                                                  rdfs:label "Ideology" .


###  http://www.ontologyrepository.com/CommonCoreOntologies/IntentionalAct
<http://www.ontologyrepository.com/CommonCoreOntologies/IntentionalAct> rdf:type owl:Class ;
                                                                        obo:IAO_0000115 "An Act in which at least one Agent plays a causative role and which is prescribed by some Directive Information Content Entity held by at least one of the Agents."@en ;
                                                                        rdfs:label "Planned Act" .


###  http://www.ontologyrepository.com/CommonCoreOntologies/MeasurementInformationContentEntity
<http://www.ontologyrepository.com/CommonCoreOntologies/MeasurementInformationContentEntity> rdf:type owl:Class ;
                                                                                             rdfs:subClassOf <http://www.ontologyrepository.com/CommonCoreOntologies/DescriptiveInformationContentEntity> ;
                                                                                             obo:IAO_0000115 "A Descriptive Information Content Entity that describes the extent, dimensions, quantity, or quality of an Entity relative to some standard."@en ;
                                                                                             rdfs:label "Measurement Information Content Entity" .


###  http://www.ontologyrepository.com/CommonCoreOntologies/PredictiveInformationContentEntity
<http://www.ontologyrepository.com/CommonCoreOntologies/PredictiveInformationContentEntity> rdf:type owl:Class ;
                                                                                            rdfs:subClassOf <http://www.ontologyrepository.com/CommonCoreOntologies/DescriptiveInformationContentEntity> ;
                                                                                            obo:IAO_0000115 "A Descriptive Information Content Entity that describes an uncertain future event."@en ;
                                                                                            rdfs:label "PredictiveInformationContentEntity" .


###  http://www.semanticweb.org/carte/ontologies/2023/6/untitled-ontology-63/FutOn:00001
<http://www.semanticweb.org/carte/ontologies/2023/6/untitled-ontology-63/FutOn:00001> rdf:type owl:Class ;
                                                                                      rdfs:subClassOf <http://www.ontologyrepository.com/CommonCoreOntologies/IntentionalAct> ;
                                                                                      obo:IAO_0000115 "an intentionalAct that represents any action deliberately performed by an individual during amatch."@en ;
                                                                                      rdfs:comment "These actions can range from playing actions (like shooting, passing, or tackling) performed by players, to strategic decisions and instructions given by coaches, to rulings and decisions made by referees."@en ;
                                                                                      rdfs:label "intentionalMatchAct"@en .


###  Generated by the OWL API (version 4.5.9.2019-02-01T07:24:44Z) https://github.com/owlcs/owlapi
